Lots of changes ,mainly about free vars
All term parts of free var substitution lemma done
Did lemmas for sub_f, sub_t
Also did lots of things for alpha sub of patterns and free vars

proofs/core/Substitution.v
@@ -1,5 +1,6 @@
 Require Import Common.
 Require Import Syntax.
+Require Import Semantics.
 Require Import Types.
 Require Import Typing.
 Require Import Denotational.
@@ -97,7 +98,8 @@ Proof.
     + rewrite skipn_length, <- H. lia.
 Qed.
 
-Context {sigma: sig}.
+Section Sub.
+Context {sigma: sig} {gamma: context} (gamma_valid: valid_context sigma gamma).
 
 
 (*Alpha substitute for patterns only in the given term/formula*)
@@ -961,6 +963,26 @@ Proof.
         apply in_split_lens_ith in Hinx; wf_tac.
 Qed.
 
+Corollary alpha_t_aux_wf (t: term):
+  (forall (l: list string),
+    NoDup l ->
+    length l = length (bnd_t t) ->
+    NoDup (bnd_t (alpha_t_aux t l)) /\
+    (forall x, In x (bnd_t (alpha_t_aux t l)) -> In (fst x) l)).
+Proof.
+  apply alpha_aux_wf_aux. apply Ftrue.
+Qed.
+
+Corollary alpha_f_aux_wf (f: formula):
+  (forall (l: list string),
+    NoDup l ->
+    length l = length (bnd_f f) ->
+    NoDup (bnd_f (alpha_f_aux f l)) /\
+    (forall x, In x (bnd_f (alpha_f_aux f l)) -> In (fst x) l)).
+Proof.
+  apply alpha_aux_wf_aux. apply tm_d.
+Qed.
+
 
 (*Need to know that all patterns in constrs are valid*)
 
@@ -1284,6 +1306,2395 @@ Proof.
     + rewrite null_map2; auto; wf_tac.
 Qed.
 
+Corollary alpha_t_aux_type (t: term) :
+  (forall (l: list string) (ty: vty)
+    (Hnodup: NoDup l)
+    (Hlenl: length l = length (bnd_t t)),
+    term_has_type sigma t ty ->
+    term_has_type sigma (alpha_t_aux t l) ty).
+Proof.
+  apply alpha_aux_valid. apply Ftrue.
+Qed.
+
+Lemma alpha_f_aux_type (f: formula):
+  (forall (l: list string)
+    (Hnodup: NoDup l)
+    (Hlenl: length l = length (bnd_f f)),
+    valid_formula sigma f ->
+    valid_formula sigma (alpha_f_aux f l)).
+Proof.
+  apply alpha_aux_valid. apply tm_d.
+Qed.
+
+Set Bullet Behavior "Strict Subproofs".
+Search sub_t term_fv.
+
+Definition set_eq {A: Type} (l1 l2: list A) : Prop :=
+  forall x, In x l1 <-> In x l2.
+
+Lemma set_eq_refl {A: Type} (l : list A) :
+  set_eq l l.
+Proof.
+  unfold set_eq; intros; reflexivity.
+Qed.
+
+Lemma set_eq_trans {A: Type} (l1 l2 l3: list A) :
+  set_eq l1 l2 ->
+  set_eq l2 l3 ->
+  set_eq l1 l3.
+Proof.
+  unfold set_eq; intros. rewrite H, H0. reflexivity.
+Qed.
+(*
+Lemma union_cons
+*)
+(*Removing from [big_union] is same as removing from each set*)
+Lemma remove_big_union {A: Type} (eq_dec: forall x y : A, {x = y} + {x <> y})
+{B: Type} (f: B -> list A) (l1: list B) (x: A) :
+set_eq (remove eq_dec x (big_union eq_dec f l1))
+  (big_union eq_dec (fun y => remove eq_dec x (f y)) l1).
+Admitted.
+
+Lemma set_eq_big_union {A: Type} (eq_dec: forall x y : A, {x = y} + {x <> y})
+  {B: Type} (f1 f2: B -> list A) (l1 l2: list B) :
+  length l1 = length l2 ->
+  Forall (fun t => set_eq (f1 (fst t)) (f2 (snd t))) (combine l1 l2) ->
+  set_eq (big_union eq_dec f1 l1) (big_union eq_dec f2 l2).
+Admitted.
+
+Ltac simpl_set_goal :=
+  repeat match goal with
+  (*remove*)
+  | H: In ?x (remove ?e ?y ?l) |- _ => rewrite in_remove_iff in H
+  | |- context [ In ?x (remove ?e ?y ?l)] => rewrite in_remove_iff
+  (*big_union*)
+  | H: In ?x (big_union ?e ?f ?l) |- _ => rewrite <- big_union_elts in H
+  | |- context [ In ?x (big_union ?e ?f ?l)] => rewrite <- big_union_elts
+  (*union*)
+  | H: In ?x (union ?e ?l1 ?l2) |- _ => rewrite union_elts in H
+  | |- context [ In ?x (union ?e ?l1 ?l2)] => rewrite union_elts
+  (*cons - TODO do without simpl*)
+  | H: In ?x (?y :: ?t) |-_ => simpl in H
+  | |- context [In ?x (?y :: ?t)] => simpl
+  (*remove \/ False from In goals*)
+  | H: ?P \/ False |- _ => rewrite or_false_r in H
+  | |- context [ ?P \/ False] => rewrite or_false_r
+  (*remove_all*)
+  | H: In ?x (remove_all ?e ?l1 ?l2) |- _ => rewrite <- remove_all_elts in H
+  | |- context [In ?x (remove_all ?e ?l1 ?l2)] => rewrite <- remove_all_elts
+  end.
+
+Ltac simpl_set :=
+  simpl_set_goal;
+  repeat match goal with
+  | H: ~ In ?x (remove_all ?e ?l1 ?l2) |- _ => revert H; simpl_set_goal; intros
+  | H: ~ In ?x (union ?e ?l1 ?l2) |- _ => revert H; simpl_set_goal; intros
+  | H: ~ In ?x (big_union ?e ?f ?l) |- _ => revert H; simpl_set_goal; intros
+  | H: ~ In ?x (remove ?e ?y ?l) |- _ => revert H; simpl_set_goal; intros
+  end.
+
+Ltac destruct_all :=
+  repeat match goal with
+  | H: ?P /\ ?Q |- _ => destruct H
+  | H: exists x, ?P |- _ => destruct H
+  | H: ?P \/ ?Q |- _ => destruct H
+  end; subst.
+
+Ltac simpl_destruct_set :=
+  repeat (progress (simpl_set; destruct_all)).
+
+Ltac triv :=
+  let inner := split_all; auto; 
+  match goal with
+  | |- ~ ?P => let C := fresh in intro C; subst; contradiction
+  end
+  in
+  try solve[inner];
+  match goal with
+  | |- ?P \/ ?Q => solve[left; inner] + solve[right; inner]
+  end.
+
+(*TODO: copied*)
+Ltac solve_bnd :=  
+  repeat match goal with
+  | H: ~In ?x (bnd_t ?t) |- ~In ?x (bnd_f ?f) =>
+    let C := fresh in
+    intro C; apply H; simpl
+  | H: ~In ?x (bnd_t ?t) |- ~In ?x (bnd_t ?t2) =>
+    let C := fresh in
+    intro C; apply H; simpl
+  | H: ~In ?x (bnd_f ?t) |- ~In ?x (bnd_f ?f) =>
+    let C := fresh in
+    intro C; apply H; simpl
+  | H: ~In ?x (bnd_f ?t) |- ~In ?x (bnd_t ?t2) =>
+    let C := fresh in
+    intro C; apply H; simpl
+  | |- In ?x (?l1 ++ ?l2) => apply in_or_app
+  | |- ?P \/ ?Q => (*idtac "x";*)
+    first [left; solve[solve_bnd] | right; solve[solve_bnd]]
+  | |- In ?x ?y => solve[try assumption; auto]
+  end.
+
+Ltac not_or name :=
+  repeat match goal with 
+  | H: ~(?P \/ ?Q) |- _ => let N1 := fresh name in
+    let N2 := fresh name in
+    apply Decidable.not_or in H;
+    
+    destruct H as [N1 N2]
+  end.
+
+Ltac case_in :=
+  repeat match goal with
+  | |- context [if in_bool ?e ?x ?l then ?y else ?z] => 
+    destruct (in_bool_spec e x l)
+  end.
+
+(*If the free var to sub is not in the term, substitution does nothing*)
+Lemma sub_notin (t: term) (f: formula) :
+  (forall (x y: vsymbol),
+    ~ In x (term_fv t) ->
+    sub_t x y t = t) /\
+    (forall (x y: vsymbol),
+    ~ In x (form_fv f) ->
+    sub_f x y f = f).
+Proof.
+  revert t f. apply term_formula_ind; simpl; auto; intros; simpl_set; not_or Hinx.
+  - destruct (vsymbol_eq_dec x v); subst; auto; contradiction.
+  - f_equal. apply list_eq_ext';
+    rewrite map_length; auto.
+    intros.
+    rewrite (map_nth_inbound) with(d2:=d); auto.
+    rewrite Forall_forall in H. apply H; wf_tac.
+    intro C. apply H0. simpl_set.  exists (nth n l1 d); split; wf_tac.
+  - rewrite H; auto.
+    destruct (vsymbol_eq_dec x v); subst; auto.
+    rewrite H0; auto.
+  - rewrite H, H0, H1; auto.
+  - rewrite H; auto. f_equal.
+    apply list_eq_ext'; rewrite map_length; auto; intros.
+    rewrite map_nth_inbound with (d2:=d); auto.
+    case_in; auto.
+    rewrite Forall_forall in H0. rewrite H0; wf_tac.
+    destruct (nth n ps d); auto.
+    intro Hinx'. apply Hinx0. exists (nth n ps d).
+    split; wf_tac. simpl_set. split; auto.
+  - destruct (vsymbol_eq_dec x v); subst; auto.
+    rewrite H; auto.
+  - f_equal. apply list_eq_ext';
+    rewrite map_length; auto.
+    intros.
+    rewrite (map_nth_inbound) with(d2:=d); auto.
+    rewrite Forall_forall in H. apply H; wf_tac.
+    intro C. apply H0.  exists (nth n tms d); split; wf_tac.
+  - destruct (vsymbol_eq_dec x v); subst; auto.
+    rewrite H; auto.
+  - rewrite H, H0; auto.
+  - rewrite H, H0; auto.
+  - rewrite H; auto.
+  - rewrite H; auto.
+    destruct (vsymbol_eq_dec x v); subst; auto.
+    rewrite H0; auto.
+  - rewrite H, H0, H1; auto.
+  - rewrite H; auto.
+    f_equal.
+    apply list_eq_ext'; rewrite map_length; auto; intros.
+    rewrite map_nth_inbound with (d2:=d); auto.
+    case_in; auto.
+    rewrite Forall_forall in H0. rewrite H0; wf_tac.
+    destruct (nth n ps d); auto.
+    intro Hinx'. apply Hinx0. exists (nth n ps d).
+    split; wf_tac. simpl_set. split; auto.
+Qed.
+
+Corollary sub_t_notin (t: term):
+  (forall (x y: vsymbol),
+    ~ In x (term_fv t) ->
+    sub_t x y t = t).
+Proof. apply sub_notin. apply Ftrue. Qed.
+
+Corollary sub_f_notin (f: formula):
+    (forall (x y: vsymbol),
+    ~ In x (form_fv f) ->
+    sub_f x y f = f).
+Proof. apply sub_notin. apply tm_d. Qed.
+
+(*If we substitute x with itself, then nothing changes*)
+Lemma sub_eq (t: term) (f: formula) :
+  (forall (x: vsymbol),
+    sub_t x x t = t) /\
+    (forall (x: vsymbol),
+    sub_f x x f = f).
+Proof.
+  revert t f; apply term_formula_ind; simpl; auto; intros.
+  - destruct (vsymbol_eq_dec x v); subst; auto.
+  - f_equal. apply list_eq_ext'; rewrite map_length; auto; intros.
+    rewrite map_nth_inbound with(d2:=d); auto.
+    rewrite Forall_forall in H; apply H; wf_tac.
+  - rewrite H. destruct (vsymbol_eq_dec x v); subst; auto.
+    rewrite H0; auto.
+  - rewrite H, H0, H1; auto.
+  - rewrite H. f_equal. apply list_eq_ext'; rewrite map_length; auto;
+    intros. rewrite map_nth_inbound with(d2:=d); auto.
+    rewrite Forall_forall in H0; rewrite H0; wf_tac.
+    case_in; auto. destruct (nth n ps d); auto.
+  - destruct (vsymbol_eq_dec x v); subst; auto. rewrite H; auto.
+  - f_equal. apply list_eq_ext'; rewrite map_length; auto; intros.
+    rewrite map_nth_inbound with(d2:=d); auto.
+    rewrite Forall_forall in H; apply H; wf_tac.
+  - destruct (vsymbol_eq_dec x v); subst; auto. rewrite H; auto.
+  - rewrite H, H0; auto.
+  - rewrite H, H0; auto.
+  - rewrite H; auto.
+  - rewrite H, H0. destruct (vsymbol_eq_dec x v); auto.
+  - rewrite H, H0, H1; auto.
+  - rewrite H. f_equal. apply list_eq_ext'; rewrite map_length; auto;
+    intros. rewrite map_nth_inbound with(d2:=d); auto.
+    rewrite Forall_forall in H0; rewrite H0; wf_tac.
+    case_in; auto. destruct (nth n ps d); auto.
+Qed.
+
+Corollary sub_t_eq (t: term):
+  (forall (x: vsymbol),
+    sub_t x x t = t).
+Proof. apply sub_eq. apply Ftrue. Qed.
+
+Corollary sub_f_eq (f: formula):
+    (forall (x: vsymbol),
+    sub_f x x f = f).
+Proof. apply sub_eq. apply tm_d. Qed.
+
+(*Alternate approach*)
+Fixpoint free_in_t (x: vsymbol) (t: term) {struct t} : bool :=
+  match t with
+  | Tconst _ => false
+  | Tvar v => vsymbol_eq_dec x v
+  | Tfun f tys tms => existsb (fun t => free_in_t x t) tms
+  | Tlet t1 v t2 =>
+    free_in_t x t1 || (negb (vsymbol_eq_dec x v) && free_in_t x t2)
+  | Tif f t1 t2 =>
+    free_in_f x f || free_in_t x t1 || free_in_t x t2
+  | Tmatch tm ty ps =>
+    free_in_t x tm ||
+    existsb (fun p => negb (in_bool vsymbol_eq_dec x (pat_fv (fst p))) &&
+      free_in_t x (snd p)) ps
+  | Teps f v => negb (vsymbol_eq_dec x v) && free_in_f x f
+  end
+with free_in_f (x: vsymbol) (f: formula) {struct f} : bool :=
+  match f with
+  | Fpred p tys tms => existsb (fun t => free_in_t x t) tms
+  | Fquant q v f1 => negb (vsymbol_eq_dec x v) && free_in_f x f1
+  | Feq ty t1 t2 => free_in_t x t1 || free_in_t x t2
+  | Fbinop b f1 f2 => free_in_f x f1 || free_in_f x f2
+  | Fnot f1 => free_in_f x f1
+  | Flet tm v f1 => free_in_t x tm || (negb (vsymbol_eq_dec x v) &&
+   free_in_f x f1)
+  | Fif f1 f2 f3 => free_in_f x f1 || free_in_f x f2 ||
+    free_in_f x f3
+  | Fmatch tm ty ps =>
+    free_in_t x tm ||
+    (existsb (fun p => negb (in_bool vsymbol_eq_dec x (pat_fv (fst p)))
+      && free_in_f x (snd p)) ps)
+  | _ => false
+  end.
+
+Ltac bool_to_prop :=
+  repeat (progress (
+  unfold is_true;
+  (*First, convert bools to props*)
+  repeat match goal with
+  | |- context [(?b && ?b1) = true] =>
+    rewrite andb_true_iff
+  | |- context [(?b1 || ?b2) = true] =>
+    rewrite orb_true_iff
+  | |- context [existsb ?f ?l = true] =>
+    rewrite existsb_exists
+  (*| |- context [negb ?b = true] =>
+    rewrite negb_true_iff*)
+  end;
+  (*Try to simplify*)
+  repeat(
+    apply or_iff_compat_l ||
+    apply and_iff_compat_l
+  );
+  (*Put the goal in a nicer form*)
+  repeat lazymatch goal with
+  | |- ?P /\ ?Q <-> ?Q /\ ?R => rewrite (and_comm P Q)
+  | |- ?P \/ ?Q <-> ?Q \/ ?R => rewrite (or_comm P Q)
+  | |- ?P /\ ?Q <-> ?R /\ ?P => rewrite (and_comm R P)
+  | |- ?P \/ ?Q <-> ?R /\ ?P => rewrite (or_comm R P)
+  | |- context [ (?P \/ ?Q) \/ ?R] => rewrite or_assoc
+  | |- ?P <-> ?P => reflexivity
+  end)).
+
+Lemma ex_in_eq {A: Type} (l: list A) (P1 P2: A -> Prop) :
+  Forall (fun x => P1 x <-> P2 x) l ->
+  (exists x, In x l /\ P1 x) <->
+  (exists x, In x l /\ P2 x).
+Proof.
+  intros. rewrite Forall_forall in H. 
+  split; intros [x [Hinx Hpx]]; exists x; split; auto;
+  apply H; auto.
+Qed.
+
+Lemma eq_sym_iff {A: Type} (x y: A):
+  x = y <-> y = x.
+Proof.
+  split; intros; subst; auto.
+Qed.
+
+Lemma dec_iff {P: Prop} {dec: {P} + { ~ P}}:
+  dec <-> P.
+Proof.
+  destruct dec; simpl; split; intros; auto. inversion H.
+Qed.
+
+Lemma dec_negb_iff {P: Prop} {dec: {P} + {~ P}}:
+  negb dec <-> ~ P.
+Proof.
+  destruct dec; simpl; split; intros; auto.
+Qed.
+(*
+destruct H.
+
+Lemma eq_dec_iff {A: Type} {eq_dec: forall (x y: A), {x = y} + {x <> y}}
+  {x y: A}:
+  eq_dec x y <-> x = y.
+Proof.
+  destruct (eq_dec x y); split; intros; subst; auto. inversion H.
+Qed.
+
+Lemma eq_dec_negb_iff  {A: Type} {eq_dec: forall (x y: A), {x = y} + {x <> y}}
+  {x y: A}:
+  negb (eq_dec x y) <-> x <> y.
+Proof.
+  destruct (eq_dec x y); split; simpl; intros; subst; simpl; auto.
+Qed.*)
+
+(*TODO: would be easier with ssreflect*)
+Lemma free_in_spec (t: term) (f: formula) :
+  (forall x, free_in_t x t <-> In x (term_fv t)) /\
+  (forall x, free_in_f x f <-> In x (form_fv f)).
+Proof.
+  revert t f.
+  apply term_formula_ind; simpl; intros; auto; simpl_set; auto;
+  try solve[split; auto].
+  - rewrite (eq_sym_iff v x), dec_iff; reflexivity. 
+  - bool_to_prop. apply ex_in_eq.
+    eapply Forall_impl. 2: apply H. simpl; intros; auto. apply H0; auto.
+  - rewrite <- H, <- H0. bool_to_prop.
+    apply dec_negb_iff.
+  - rewrite<- H, <- H0, <- H1.
+    bool_to_prop.
+  - rewrite <- H. bool_to_prop.
+    apply ex_in_eq.
+    revert H0. rewrite !Forall_forall; intros. simpl_set.
+    bool_to_prop.
+    rewrite <- H0; wf_tac. bool_to_prop.
+    rewrite <- in_bool_dec.
+    apply dec_negb_iff.
+  - rewrite <- H; bool_to_prop.
+    apply dec_negb_iff.
+  - bool_to_prop. apply ex_in_eq.
+    eapply Forall_impl. 2: apply H. simpl; intros; auto. apply H0; auto.
+  - rewrite <- H; bool_to_prop. apply dec_negb_iff.
+  - rewrite <- H, <- H0. bool_to_prop.
+  - rewrite <- H, <- H0; bool_to_prop.
+  - rewrite <- H, <- H0; bool_to_prop.
+    apply dec_negb_iff.
+  - rewrite <- H, <- H0, <- H1; bool_to_prop.
+  - rewrite <- H. bool_to_prop.
+    apply ex_in_eq.
+    revert H0. rewrite !Forall_forall; intros. simpl_set.
+    bool_to_prop.
+    rewrite <- H0; wf_tac. bool_to_prop.
+    rewrite <- in_bool_dec.
+    apply dec_negb_iff.
+Qed.
+
+Corollary free_in_t_spec (t: term):
+(forall x, free_in_t x t <-> In x (term_fv t)).
+Proof. apply free_in_spec. apply Ftrue. Qed.
+
+Lemma free_in_t_negb (t: term):
+forall x, free_in_t x t = false <-> ~In x (term_fv t).
+Proof.
+  intros. destruct (free_in_t x t) eqn : Hfree; split; intros; auto.
+  assert (is_true (free_in_t x t)) by auto.
+  apply free_in_t_spec in H0. contradiction.
+  intro Hin. apply free_in_t_spec in Hin.
+  rewrite Hfree in Hin. inversion Hin.
+Qed.
+
+Corollary free_in_f_spec (f: formula):
+(forall x, free_in_f x f <-> In x (form_fv f)).
+Proof. apply free_in_spec. apply tm_d. Qed.
+
+Lemma free_in_f_negb (f: formula):
+forall x, free_in_f x f = false <-> ~In x (form_fv f).
+Proof.
+  intros. destruct (free_in_f x f) eqn : Hfree; split; intros; auto.
+  assert (is_true (free_in_f x f)) by auto.
+  apply free_in_f_spec in H0. contradiction.
+  intro Hin. apply free_in_f_spec in Hin.
+  rewrite Hfree in Hin. inversion Hin.
+Qed.
+
+(*Now we can reason about [free_in]*)
+
+(*3 lemmas about free vars and [sub_t]*)
+
+Ltac vsym_eq x y :=
+  destruct (vsymbol_eq_dec x y); subst; auto; try contradiction.
+
+Lemma existsb_eq {A: Type} {f1 f2: A -> bool} (l1 l2: list A):
+  length l1 = length l2 ->
+  Forall (fun x => f1 (fst x) = f2 (snd x)) (combine l1 l2) ->
+  existsb f1 l1 = existsb f2 l2.
+Proof.
+  revert l2. induction l1; simpl; intros; destruct l2; inversion H; simpl; auto.
+  inversion H0; subst.
+  simpl in H4. rewrite H4, (IHl1 l2); auto.
+Qed. 
+  
+
+(*1. For any variables which are not x or y, sub_t doesn't change anything*)
+Lemma sub_fv_diff (t: term) (f: formula):
+  (forall (x y z: vsymbol),
+    z <> x -> z <> y ->
+    free_in_t z (sub_t x y t) = free_in_t z t) /\
+  (forall (x y z: vsymbol),
+    z <> x -> z <> y ->
+    free_in_f z (sub_f x y f) = free_in_f z f).
+Proof.
+  revert t f.
+  apply term_formula_ind; simpl; auto; intros.
+  - vsym_eq x v. vsym_eq z y. vsym_eq z v.
+  - apply existsb_eq; wf_tac.
+    revert H. rewrite !Forall_forall; intros.
+    revert H2. 
+    rewrite in_combine_iff; wf_tac.
+    intros [i [Hi Hx]]. specialize (Hx tm_d tm_d); subst; simpl.
+    wf_tac.
+    apply H; wf_tac.
+  - rewrite H; auto. f_equal. f_equal.
+    vsym_eq x v.
+  - rewrite H, H0, H1; auto.
+  - rewrite H; auto. f_equal.
+    apply existsb_eq; wf_tac.
+    revert H0.
+    rewrite !Forall_forall; intros.
+    revert H3.
+    rewrite in_combine_iff; wf_tac.
+    intros [i [Hi Hx]]; specialize (Hx (Pwild, tm_d) (Pwild, tm_d)); subst; simpl.
+    wf_tac. case_in; auto.
+    simpl; rewrite H0; wf_tac.
+  - vsym_eq x v. simpl. rewrite H; auto.
+  - apply existsb_eq; wf_tac.
+    revert H. rewrite !Forall_forall; intros.
+    revert H2. 
+    rewrite in_combine_iff; wf_tac.
+    intros [i [Hi Hx]]. specialize (Hx tm_d tm_d); subst; simpl.
+    wf_tac.
+    apply H; wf_tac.
+  - vsym_eq x v; simpl; rewrite H; auto.
+  - rewrite H, H0; auto.
+  - rewrite H, H0; auto.
+  - rewrite H; auto. f_equal. f_equal.
+    vsym_eq x v.
+  - rewrite H, H0, H1; auto.
+  - rewrite H; auto. f_equal.
+    apply existsb_eq; wf_tac.
+    revert H0.
+    rewrite !Forall_forall; intros.
+    revert H3.
+    rewrite in_combine_iff; wf_tac.
+    intros [i [Hi Hx]]; specialize (Hx (Pwild, Ftrue) (Pwild, Ftrue)); subst; simpl.
+    wf_tac. case_in; auto.
+    simpl; rewrite H0; wf_tac.
+Qed.
+
+Corollary sub_t_fv_diff (t: term):
+  (forall (x y z: vsymbol),
+    z <> x -> z <> y ->
+    free_in_t z (sub_t x y t) = free_in_t z t).
+Proof. apply sub_fv_diff. apply Ftrue. Qed.
+
+Corollary sub_f_fv_diff (f:formula):
+  (forall (x y z: vsymbol),
+    z <> x -> z <> y ->
+    free_in_f z (sub_f x y f) = free_in_f z f).
+Proof. apply sub_fv_diff. apply tm_d. Qed.
+
+Lemma existsb_false {A: Type} (f: A -> bool) (l: list A):
+  (existsb f l = false) <-> Forall (fun x => f x = false) l.
+Proof.
+  induction l; simpl; split; intros; auto.
+  - rewrite orb_false_iff in H.
+    destruct_all; subst; constructor; auto.
+    apply IHl; auto.
+  - rewrite orb_false_iff. inversion H; subst.
+    split; auto. apply IHl; auto.
+Qed.
+
+(*2: If we replace x with y, x is NOT in the resulting free variables*)
+Lemma sub_fv_notin (t: term) (f: formula):
+  (forall (x y: vsymbol),
+    x <> y ->
+    free_in_t x (sub_t x y t) = false) /\
+  (forall (x y: vsymbol),
+    x <> y ->
+    free_in_f x (sub_f x y f) = false).
+Proof.
+  revert t f. apply term_formula_ind; simpl; auto; intros.
+  - vsym_eq x v. vsym_eq v y. vsym_eq x v.
+  - apply existsb_false.
+    revert H. rewrite !Forall_forall; intros.
+    revert H1. rewrite in_map_iff; intros [t [Ht Hint]]; subst.
+    apply H; auto.
+  - rewrite !orb_false_iff. split; [apply H; auto|].
+    vsym_eq x v. simpl. apply H0; auto.
+  - rewrite H, H0, H1; auto.
+  - rewrite H; simpl; auto.
+    apply existsb_false. revert H0. rewrite !Forall_forall; intros.
+    revert H2. rewrite in_map_iff; intros [p1 [Hp1 Hinp1]]; subst.
+    case_in; simpl; destruct (in_bool_spec vsymbol_eq_dec x (pat_fv (fst p1))); simpl; auto;
+    try contradiction.
+    apply H0; wf_tac.
+  - vsym_eq x v; simpl; auto. vsym_eq v v.
+    vsym_eq x v; simpl. apply H; auto.
+  - apply existsb_false.
+    revert H. rewrite !Forall_forall; intros.
+    revert H1. rewrite in_map_iff; intros [t [Ht Hint]]; subst.
+    apply H; auto.
+  - vsym_eq x v; simpl. vsym_eq v v. vsym_eq x v; simpl.
+    apply H; auto.
+  - rewrite H, H0; auto.
+  - rewrite H, H0; auto.
+  - rewrite H; auto; simpl. vsym_eq x v; simpl.
+    apply H0; auto.
+  - rewrite H, H0, H1; auto.
+  - rewrite H; simpl; auto.
+    apply existsb_false. revert H0. rewrite !Forall_forall; intros.
+    revert H2. rewrite in_map_iff; intros [p1 [Hp1 Hinp1]]; subst.
+    case_in; simpl; destruct (in_bool_spec vsymbol_eq_dec x (pat_fv (fst p1))); simpl; auto;
+    try contradiction.
+    apply H0; wf_tac.
+Qed.
+
+Corollary sub_t_fv_notin (t: term):
+  (forall (x y: vsymbol),
+    x <> y ->
+    free_in_t x (sub_t x y t) = false).
+Proof. apply sub_fv_notin. apply Ftrue. Qed.
+
+Corollary sub_f_fv_notin (f: formula):
+  (forall (x y: vsymbol),
+    x <> y ->
+    free_in_f x (sub_f x y f) = false).
+Proof. apply sub_fv_notin. apply tm_d. Qed.
+
+Lemma existsb_orb {A: Type} (f1 f2: A -> bool) (l: list A):
+  existsb f1 l || existsb f2 l =
+  existsb (fun x => f1 x || f2 x) l.
+Proof.
+  induction l; simpl; auto.
+  rewrite <- !orb_assoc. f_equal.
+  rewrite orb_comm, <- orb_assoc. f_equal.
+  rewrite orb_comm; apply IHl.
+Qed.
+
+Ltac simpl_bool :=
+  repeat (progress (simpl;
+  try rewrite !orb_assoc;
+  try rewrite !andb_assoc;
+  repeat match goal with
+  | |- context [ ?b && true] => rewrite andb_true_r
+  | |- context [?b || true] => rewrite orb_true_r
+  | |- context [?b && false] => rewrite andb_false_r
+  | |- context [?b || false] => rewrite orb_false_r
+  end)).
+
+Ltac solve_bool :=
+  simpl_bool;
+  (*Then brute force the solution*)
+  repeat 
+  (match goal with
+  | |- ?b1 && ?b2 = ?z => destruct b2
+  | |- ?b1 || ?b2 = ?z => destruct b2
+  | |- ?z = ?b1 && ?b2 => destruct b2
+  | |- ?z = ?b1 || ?b2 => destruct b2
+  end; simpl_bool; try reflexivity).
+
+
+(*3. When we substitute x with y, y is in the free variables
+  iff either y was before or x was before*)
+(*Need the Hbnd assumption for the following: in let t1 = v in t2,
+  if y =v, then y will not be in the free variables of
+  the substituted term even if x is a free variable in t2*)
+Lemma sub_fv_in (t: term) (f: formula):
+  (forall (x y: vsymbol)
+    (Hbnd: ~ In y (bnd_t t)),
+    x <> y ->
+    free_in_t y (sub_t x y t) = (free_in_t x t) || (free_in_t y t)) /\
+  (forall (x y: vsymbol)
+    (Hbnd: ~ In y (bnd_f f)),
+    x <> y ->
+    free_in_f y (sub_f x y f) = (free_in_f x f) || (free_in_f y f)).
+Proof.
+  revert t f. apply term_formula_ind; simpl; auto; intros.
+  - vsym_eq x v; simpl.
+    vsym_eq y y.
+  - rewrite existsb_orb.
+    apply existsb_eq; wf_tac.
+    revert H. rewrite !Forall_forall; intros.
+    revert H1. rewrite in_combine_iff; wf_tac.
+    intros [i [Hi Hx]]. specialize (Hx tm_d tm_d); subst; simpl.
+    wf_tac. apply H; wf_tac. intro C.
+    apply Hbnd. rewrite in_concat. exists (bnd_t (nth i l1 tm_d)); 
+    split; wf_tac.
+  - rewrite H; auto; [|intro C; apply Hbnd; right; apply in_or_app; triv]. 
+    rewrite <- !orb_assoc. f_equal.
+    rewrite !orb_andb_distrib_r.
+    vsym_eq x v.
+    rewrite H0; auto; [|intro C; apply Hbnd; right; apply in_or_app; triv].
+    vsym_eq y v. exfalso. apply Hbnd; triv.
+    simpl. solve_bool.
+  - rewrite H, H0, H1; auto;[solve_bool| | |]; intro C; apply Hbnd;
+    rewrite !in_app_iff; triv.
+  - (*match is hard case not surprisingly*)
+    rewrite H; auto; [|intro C; apply Hbnd; rewrite in_app_iff; triv].
+    simpl_bool. rewrite (orb_comm (_ || _) (free_in_t y tm)).
+    rewrite orb_assoc, (orb_comm (free_in_t y tm)).
+    rewrite <- !orb_assoc. f_equal. f_equal.
+    (*Now just have the exists goal*)
+    rewrite existsb_orb.
+    apply existsb_eq; wf_tac.
+    revert H0. rewrite !Forall_forall; intros.
+    revert H2. rewrite in_combine_iff; wf_tac; intros [i [Hi Hx]].
+    specialize (Hx (Pwild, tm_d) (Pwild, tm_d)); subst; simpl.
+    wf_tac. case_in; simpl; auto.
+    destruct (in_bool_spec vsymbol_eq_dec y (pat_fv (fst (nth i ps (Pwild, tm_d))))); simpl.
+    + (*contradiction: y not in bound vars*)
+      exfalso. apply Hbnd. rewrite in_app_iff. right.
+      rewrite in_concat. exists ((pat_fv (fst (nth i ps (Pwild, tm_d))))
+      ++ (bnd_t (snd (nth i ps (Pwild, tm_d))))).
+      split; wf_tac. exists (nth i ps (Pwild, tm_d)). split; wf_tac.
+      rewrite in_app_iff; triv.
+    + rewrite H0; wf_tac. intro C.
+      apply Hbnd. rewrite in_app_iff. right. 
+      rewrite in_concat. exists ((pat_fv (fst (nth i ps (Pwild, tm_d))))
+      ++ (bnd_t (snd (nth i ps (Pwild, tm_d))))).
+      split; wf_tac. exists (nth i ps (Pwild, tm_d)). split; wf_tac.
+      rewrite in_app_iff; triv.
+  - vsym_eq x v; simpl.
+    vsym_eq y v; simpl.
+    + exfalso; apply Hbnd; triv.
+    + rewrite H; auto.
+  - rewrite existsb_orb.
+    apply existsb_eq; wf_tac.
+    revert H. rewrite !Forall_forall; intros.
+    revert H1. rewrite in_combine_iff; wf_tac.
+    intros [i [Hi Hx]]. specialize (Hx tm_d tm_d); subst; simpl.
+    wf_tac. apply H; wf_tac. intro C.
+    apply Hbnd. rewrite in_concat. exists (bnd_t (nth i tms tm_d)); 
+    split; wf_tac.
+  - vsym_eq x v; simpl.
+    vsym_eq y v; simpl.
+    + exfalso; apply Hbnd; triv.
+    + rewrite H; auto.
+  - rewrite H, H0; auto; [solve_bool | |]; intro C; apply Hbnd;
+    rewrite in_app_iff; triv.
+  - rewrite H, H0; auto; [solve_bool | |]; intro C; apply Hbnd;
+    rewrite in_app_iff; triv.
+  - rewrite H; auto; [|intro C; apply Hbnd; right; apply in_or_app; triv]. 
+    rewrite <- !orb_assoc. f_equal.
+    rewrite !orb_andb_distrib_r.
+    vsym_eq x v.
+    rewrite H0; auto; [|intro C; apply Hbnd; right; apply in_or_app; triv].
+    vsym_eq y v. exfalso. apply Hbnd; triv.
+    simpl. solve_bool.
+  - rewrite H, H0, H1; auto;[solve_bool | | |]; intro C;
+    apply Hbnd; rewrite !in_app_iff; triv.
+  - rewrite H; auto; [|intro C; apply Hbnd; rewrite in_app_iff; triv].
+    simpl_bool. rewrite (orb_comm (_ || _) (free_in_t y tm)).
+    rewrite orb_assoc, (orb_comm (free_in_t y tm)).
+    rewrite <- !orb_assoc. f_equal. f_equal.
+    (*Now just have the exists goal*)
+    rewrite existsb_orb.
+    apply existsb_eq; wf_tac.
+    revert H0. rewrite !Forall_forall; intros.
+    revert H2. rewrite in_combine_iff; wf_tac; intros [i [Hi Hx]].
+    specialize (Hx (Pwild, Ftrue) (Pwild, Ftrue)); subst; simpl.
+    wf_tac. case_in; simpl; auto.
+    destruct (in_bool_spec vsymbol_eq_dec y (pat_fv (fst (nth i ps (Pwild, Ftrue))))); simpl.
+    + (*contradiction: y not in bound vars*)
+      exfalso. apply Hbnd. rewrite in_app_iff. right.
+      rewrite in_concat. exists ((pat_fv (fst (nth i ps (Pwild, Ftrue))))
+      ++ (bnd_f (snd (nth i ps (Pwild, Ftrue))))).
+      split; wf_tac. exists (nth i ps (Pwild, Ftrue)). split; wf_tac.
+      rewrite in_app_iff; triv.
+    + rewrite H0; wf_tac. intro C.
+      apply Hbnd. rewrite in_app_iff. right. 
+      rewrite in_concat. exists ((pat_fv (fst (nth i ps (Pwild, Ftrue))))
+      ++ (bnd_f (snd (nth i ps (Pwild, Ftrue))))).
+      split; wf_tac. exists (nth i ps (Pwild, Ftrue)). split; wf_tac.
+      rewrite in_app_iff; triv.
+Qed. 
+
+Corollary sub_t_fv_in (t: term):
+  (forall (x y: vsymbol)
+    (Hbnd: ~ In y (bnd_t t)),
+    x <> y ->
+    free_in_t y (sub_t x y t) = (free_in_t x t) || (free_in_t y t)). 
+Proof. apply sub_fv_in. apply Ftrue. Qed.
+
+Corollary sub_f_fv_in (f: formula):
+  (forall (x y: vsymbol)
+    (Hbnd: ~ In y (bnd_f f)),
+    x <> y ->
+    free_in_f y (sub_f x y f) = (free_in_f x f) || (free_in_f y f)).
+Proof. apply sub_fv_in. apply tm_d. Qed.
+
+(*Analagous lemmas for term/formula in [alpha_p_aux]*)
+
+(*1. For any vsymbol not in the free vars of p and not
+  in the image of the free variables in l, 
+  [alpha_p_aux] does not change the result*)
+(*TODO: is (notin (map snd l)) too strong? Should be ok i think*)
+
+Lemma alpha_p_aux_diff {A: Type} (sub: vsymbol -> vsymbol -> A -> A)
+(p: pattern) (t: A) (l: list (vsymbol * string))
+(free_in: vsymbol -> A -> bool)
+(Hsub: forall a x y z, z <> x -> z <> y -> 
+  free_in z (sub x y a) = free_in z a)
+(Hnodup: NoDup(map fst l))
+(Hallin: forall v, In v (pat_fv p) -> In v (map fst l)):
+forall x, ~In x (pat_fv p) ->
+  ~ In x (pat_fv (fst (alpha_p_aux sub p t l))) ->
+   free_in x (snd (alpha_p_aux sub p t l)) = free_in x t.
+Proof.
+  intros x.
+  (*This makes it usable with our IH for constr case*)
+  rewrite alpha_p_aux_wf_aux_gen'; auto.
+  generalize dependent t.
+  induction p; simpl in *; intros; auto.
+  - destruct (get_assoc_list vsymbol_eq_dec l v) eqn : ha; auto.
+    simpl. rewrite Hsub; auto.
+    intro Heq; subst.
+    apply get_assoc_list_some in ha.
+    apply H0. simpl. exists v. exists s. split_all; auto.
+  - generalize dependent t. induction ps; simpl; intros; auto.
+    inversion H; subst.
+    rewrite IHps; auto.
+    + simpl in H0. simpl_set. rewrite H4; auto.
+      * intros. apply Hallin. simpl; simpl_set; triv.
+      * intros [v [str [Hinvst [Hinv [Hsnd Hfst]]]]]; subst.
+        apply H1. exists v. exists (fst x). split_all; auto.
+        simpl; simpl_set; triv.
+    + intros. apply Hallin. simpl; simpl_set; triv.
+    + simpl in H0. rewrite union_elts in H0.
+      intro C. apply H0. triv.
+    + intros [v [str [Hinvstr [Hinv [Hsnd Hfst]]]]]; subst.
+      apply H1. exists v. exists (fst x). split_all; auto.
+      simpl. simpl_set; triv.
+  - rewrite IHp2; auto.
+    + intros. apply Hallin. simpl_set; triv.
+    + intro C. apply H. simpl_set; triv.
+    + intros [v [str [Hinv1 [Hinv2 [Hfst Hsnd]]]]]; subst.
+      apply H0. exists v. exists (fst x). split_all; auto.
+      simpl_set; triv.
+  - destruct (get_assoc_list vsymbol_eq_dec l v) eqn : Ha; auto.
+    simpl. rewrite Hsub; auto.
+    + apply IHp.
+      * intros; apply Hallin; simpl_set; triv.
+      * intro C. apply H. simpl_set; triv.
+      * intros [v' [str [Hinv1 [Hinv2 [Hfst Hsnd]]]]]; subst.
+        apply H0. exists v'. exists (fst x). split_all; auto.
+        simpl_set; triv.
+    + intro Heq; subst. apply H. simpl_set; triv.
+    + intro Heq; subst. apply H0. simpl.
+      apply get_assoc_list_some in Ha.
+      exists v. exists s. split_all; auto. simpl_set; triv.
+Qed.
+(*
+Lemma alpha_p_aux_diff {A: Type} (sub: vsymbol -> vsymbol -> A -> A)
+(p: pattern) (t: A) (l: list (vsymbol * string))
+(free_in: vsymbol -> A -> bool)
+(Hsub: forall a x y z, z <> x -> z <> y -> 
+  free_in z (sub x y a) = free_in z a):
+forall x, ~In x (pat_fv p) ->
+  ~ In (fst x) (map snd l) ->
+   free_in x (snd (alpha_p_aux sub p t l)) = free_in x t.
+Proof.
+  intros. revert t.
+  induction p; simpl in *; intros.
+  - destruct (get_assoc_list vsymbol_eq_dec l v) eqn : ha.
+    + simpl. rewrite Hsub; auto.
+      intro Heq; subst.
+      apply get_assoc_list_some in ha.
+      apply H0. rewrite in_map_iff; simpl.
+      exists (v, s). split; auto.
+    + auto.
+  - generalize dependent t. induction ps; simpl; intros; auto.
+    inversion H1; subst.
+    rewrite IHps; auto.
+    + rewrite H4; auto.
+      intro C. apply H. simpl. simpl_set. triv.
+    + intro C. apply H. simpl. simpl_set. triv.
+  - auto.
+  - rewrite IHp2; auto.
+    intro C. apply H. simpl_set; triv.
+  - destruct (get_assoc_list vsymbol_eq_dec l v) eqn : Ha.
+    + simpl. rewrite Hsub; auto.
+      * apply IHp.
+        intro C. apply H. simpl_set; triv.
+      * intro Heq; subst. apply H. simpl_set; triv.
+      * intro Heq; subst. apply H0. simpl.
+        apply get_assoc_list_some in Ha.
+        rewrite in_map_iff. exists (v, s); auto.
+    + auto.
+Qed.
+
+(*Version that uses only free vars in patterns before and after.
+  Need a lot of assumptions about list l*)
+Lemma alpha_p_aux_diff' {A: Type} (sub: vsymbol -> vsymbol -> A -> A)
+(p: pattern) (t: A) (l: list (vsymbol * string))
+(free_in: vsymbol -> A -> bool)
+(Hsub: forall a x y z, z <> x -> z <> y -> 
+  free_in z (sub x y a) = free_in z a)
+(Hnodup: NoDup (map fst l))
+(Hallfv1: forall x y, In (x, y) l -> In x (pat_fv p))
+(Hallfv2: forall v, In v (pat_fv p) -> In v (map fst l)):
+forall x, ~In x (pat_fv p) ->
+  ~ In (fst x) (map fst (pat_fv (fst (alpha_p_aux sub p t l)))) ->
+   free_in x (snd (alpha_p_aux sub p t l)) = free_in x t.
+Proof.
+  intros. apply alpha_p_aux_diff; auto.
+  intro Hinl. apply H0.
+  rewrite in_map_iff in Hinl.
+  assert (~ In x (pat_fv (fst (alpha_p_aux sub p t l)))). admit.
+  clear H0.
+  assert (~In (fst x) (map fst (pat_fv (fst (alpha_p_aux sub p t l))))).
+  intro C.
+  (*apply H1.*) rewrite in_map_iff in C. destruct 
+  C as [y [Hfst Hiny]].
+
+  
+  
+  rewrite in_map_iff in H1.
+  intro C. apply H0. rewrite in_map_iff.
+  exists x. split; auto.
+  (*Hmm need to think
+    So is the stronger statement true?
+    The free vars that are affected are the ones in (pat_fv p)
+      (which are replaced) and the ones in (pat_fv (fst ...)),
+      which are substituted for
+    The problem becomes: what if x has the same name as something
+    that is in the free vars,
+    so we have y in resulting pat_fv, x notin resulting pat_fv
+    this means that y is in (map snd l)
+
+    
+    If x is not in resulting free vars, then
+
+  
+  *)
+  apply alpha_p_aux_wf_aux_gen'; auto.
+  rewrite in_map_iff in Hinl.
+  destruct Hinl as [y [Hfst Hy]].
+  destruct y as [v str].
+  assert (Hy':=Hy).
+  apply Hallfv1 in Hy.
+  simpl in *; subst.
+  exists v. exists (fst x). split_all; auto.
+  
+  
+  exists str. split_all; auto.
+  exists (v, str).
+  simpl in Hfst; subst.
+  assert (Hy':=Hy).
+  apply Hallfv1 in Hy.
+  rewrite in_map_iff.
+  exists (fst x, snd v). split; auto.
+  rewrite alpha_p_aux_wf_aux_gen'; auto.
+  exists v. exists (fst x). auto.
+Qed.*)
+
+
+Lemma sub_t_in_implies (t: term): forall z x y,
+  free_in_t z (sub_t x y t) ->
+  (free_in_t z t /\ z <> x) \/ z = y.
+Proof.
+  intros. vsym_eq x y.
+  - rewrite sub_t_eq in H. vsym_eq z y.
+  - vsym_eq z x.
+    + rewrite (sub_t_fv_notin _ _ _ n) in H. inversion H.
+    + vsym_eq z y.
+      rewrite sub_t_fv_diff in H; auto.
+Qed.
+(*Let's see:
+  every variable free in the result is free in the term or
+  is in the image of the list*)
+  (*TODO: add pattern well typed for or case*)
+Lemma alpha_p_aux_in_implies {A: Type} (sub: vsymbol -> vsymbol -> A -> A)
+  (p: pattern) (t: A) (l: list (vsymbol * string))
+  (free_in: vsymbol -> A -> bool) (ty: vty)
+  (Hty: pattern_has_type sigma p ty)
+  (Hsub: forall z x y a, free_in z (sub x y a) ->
+    (free_in z a /\ z <> x) \/ z = y)
+  (Hallin: forall x, In x (pat_fv p) -> In x (map fst l))
+  (Hnodup: NoDup (map fst l)) :
+  forall x, free_in x (snd (alpha_p_aux sub p t l)) ->
+    (free_in x t /\ ~In x (pat_fv p)) \/ 
+      In x (pat_fv(fst (alpha_p_aux sub p t l))).
+Proof.
+  intros.
+  rewrite alpha_p_aux_wf_aux_gen'; auto.
+  intros; generalize dependent ty; generalize dependent t; induction p; simpl in *; intros.
+  - destruct (get_assoc_list vsymbol_eq_dec l v) eqn : Ha;
+    simpl in H.
+    + apply Hsub in H. destruct H as [[Hfree Hneq] | Heq]; subst; try triv.
+      * left. split; auto. intro C; destruct_all; subst; auto; try contradiction.
+      * right. simpl. exists v. exists s. split_all; auto.
+        apply get_assoc_list_some in Ha; auto.
+    + apply get_assoc_list_none in Ha. exfalso. apply Ha. apply Hallin.
+      triv. 
+  - generalize dependent t.
+    inversion Hty; subst.
+    revert H9. clear H3 H4 H7 H10 Hty.
+    assert (length ps = length (map sigma0 (s_args f))) by (rewrite map_length; auto).
+    revert H0; clear H5.
+    generalize dependent (map sigma0 (s_args f)).
+    induction ps; simpl; intros; auto.
+    inversion H; subst.
+    destruct l0; inversion H0.
+    inversion H9; subst. simpl in H7.
+    eapply IHps in H1; auto. 3: apply H3.
+    + destruct H1.
+      * destruct H1. eapply H4 in H1. 3: apply H7.
+        -- destruct H1.
+          ++ destruct H1. left. split; auto.
+            simpl_set. intro C. destruct C; contradiction.
+          ++ right. destruct H1 as [v' [str[Hinv1 [Hinv2 [Hfst Hsnd]]]]]; subst.
+            exists v'. exists (fst x). split_all; auto.
+            simpl_set; triv.
+        -- intros; apply Hallin; simpl; simpl_set; triv.
+      * right. destruct H1 as [v' [str[Hinv1 [Hinv2 [Hfst Hsnd]]]]]; subst.
+        exists v'. exists (fst x). split_all; auto. simpl_set; triv.
+    + intros; apply Hallin; simpl; simpl_set; triv.
+    + auto. 
+  - triv. 
+  - inversion Hty; subst. 
+    eapply IHp2 in H. 3: apply H4.
+    + destruct H; try triv.
+      * destruct H. left. split; auto. simpl_set.
+        intros [Hinx | Hinx]; try contradiction.
+        (*Need typing to know that free vars the same*)
+        rewrite H6 in Hinx. contradiction.
+      * right. destruct H as [v' [str[Hinv1 [Hinv2 [Hfst Hsnd]]]]]; subst.
+        exists v'; exists (fst x); split_all; auto; simpl_set; triv.
+    + intros; apply Hallin; simpl; simpl_set; triv.
+  - inversion Hty; subst. 
+    destruct (get_assoc_list vsymbol_eq_dec l v) eqn : Ha;
+    simpl in H.
+    + apply Hsub in H. destruct H; subst; simpl; try triv.
+      * destruct H. eapply IHp in H. 3: apply H5.
+        -- destruct_all; try triv.
+          ++ left.
+            split; auto; simpl_set. intros [C | C]; subst; auto.
+          ++ right. exists x0. exists (fst x). split_all; auto. simpl_set; triv. 
+        -- intros; apply Hallin; simpl; simpl_set; triv.
+      * right. apply get_assoc_list_some in Ha.
+        exists v. exists s. split_all; auto. simpl_set. triv.
+    + apply get_assoc_list_none in Ha.
+      exfalso. apply Ha. apply Hallin. simpl_set. triv.
+Qed.
+
+(*2. For any vsymbol in the free vars of p, it is not free
+  in the result*)
+Lemma alpha_p_aux_notin {A: Type} (sub: vsymbol -> vsymbol -> A -> A)
+  (p: pattern) (t: A) (l: list (vsymbol * string))
+  (free_in: vsymbol -> A -> bool) ty
+  (Hty: pattern_has_type sigma p ty)
+  (Hsub1: forall x y a, x <> y -> free_in x (sub x y a) = false)
+  (Hsub2: forall z x y a, free_in z (sub x y a) ->
+    (free_in z a /\ z <> x) \/ z = y)
+  (Hfree: forall x, In (fst x) (map snd l) -> ~ In x (pat_fv p))
+  (Hallin: forall x, In x (pat_fv p) -> In x (map fst l))
+  (Hnodup: NoDup (map fst l)):
+  forall x, In x (pat_fv p) ->
+  ~In x (pat_fv (fst (alpha_p_aux sub p t l))) ->
+  free_in x (snd (alpha_p_aux sub p t l)) = false.
+Proof.
+  intros. rewrite alpha_p_aux_wf_aux_gen' in H0; auto.
+  generalize dependent ty. 
+  generalize dependent t.
+  induction p; intros; simpl in H; simpl.
+  - destruct H as [Heq | []]; subst.
+    destruct (get_assoc_list vsymbol_eq_dec l x) eqn : Ha.
+    + simpl. apply Hsub1. intro Hx.
+      apply (Hfree x); simpl; try triv.
+      rewrite Hx. simpl.
+      apply get_assoc_list_some in Ha.
+      rewrite in_map_iff. exists (x, s); auto.
+    + apply get_assoc_list_none in Ha.
+      exfalso. apply Ha. apply Hallin; simpl; triv.
+  - assert (In x (big_union vsymbol_eq_dec pat_fv ps) \/ free_in x t = false) by triv.
+    clear H. (*Need weaker statement for IH*)
+    inversion Hty; subst.
+    revert H11. clear H5 H6 H9 H12 Hty.
+    assert (length ps = length (map sigma0 (s_args f))) by (rewrite map_length; auto).
+    revert H; clear H7.
+    generalize dependent (map sigma0 (s_args f)). clear sigma0.
+    generalize dependent t.  induction ps; simpl; intros; auto.
+    + destruct H2 as [[] |]; auto.
+    + simpl in *.
+      destruct l0; inversion H.
+      inversion H11; subst. simpl in H6.
+    (*TODO: think need separate lemma for base case see*)
+      destruct H2.
+      * inversion H1; subst. eapply IHps; [| | | | |apply H4 |]; auto.
+        -- intros y Hiny C.
+          apply (Hfree y); auto. simpl_set; triv.
+        -- intros. apply Hallin. simpl_set; triv.
+        -- intros [v' [str [Hinv1 [Hinv2 [Hsnd Hfst]]]]]; subst.
+          apply H0. exists v'. exists (fst x). split_all; auto.
+          simpl_set; triv.
+        -- rewrite union_elts in H2.
+          destruct H2.
+          (*Why we need weaker IH*)
+          ++ right. eapply H8; [| | | | apply H6]; auto.
+            ** intros y Hiny C.
+              apply (Hfree y); auto. simpl_set; triv.
+            ** intros; apply Hallin; simpl_set; triv.
+            ** intros [v' [str [Hinv1 [Hinv2 [Hsnd Hfst]]]]]; subst.
+              apply H0. exists v'. exists (fst x). split_all; auto.
+              simpl_set; triv.
+          ++ left; auto.
+      * (*Prove this by separate inductive lemma - this is annoying*)
+        (*We need to prove this part twice - can we improve?*)
+        destruct (free_in x (snd (alpha_p_aux sub a t l))) eqn : Hfreext.
+        {
+          eapply alpha_p_aux_in_implies in Hfreext; [| apply H6 | | |]; auto.
+          - exfalso. destruct Hfreext.
+            + destruct H3; rewrite H3 in H2; inversion H2.
+            + rewrite alpha_p_aux_wf_aux_gen' in H3; auto.
+              apply H0. destruct H3 as [v' [str [Hinv1 [Hinv2 [Hsnd Hfst]]]]]; subst.
+              exists v'. exists (fst x). split_all; auto. 
+              simpl_set; triv.
+              intros; apply Hallin. simpl_set; triv.
+          - intros. apply Hallin. simpl_set; triv.
+          }
+        (*Also need to know type*)
+        generalize dependent (snd (alpha_p_aux sub a t l)).
+        revert H7. revert H4. 
+        assert (~
+        (exists (v : vsymbol) (str : string),
+           In (v, str) l /\
+           In v
+                (big_union vsymbol_eq_dec pat_fv ps) /\
+           snd x = snd v /\ fst x = str)). {
+            intros [v' [str [Hinv1 [Hinv2 [Hfst Hsnd]]]]]; subst.
+            apply H0. exists v'. exists (fst x). split_all; auto.
+            simpl_set; triv.
+           }
+          revert H3.
+          clear -sigma Hnodup Hallin Hsub2. (*TODO: see if we need anything*)
+          revert l0.
+          induction ps; simpl; intros; auto.
+          destruct l0; inversion H4.
+          inversion H7; subst.
+          eapply IHps; [| | apply H0 | |]; auto.
+          -- intros. apply Hallin. simpl. simpl_set. 
+            destruct H; try triv. simpl_set. triv.
+          -- intros [v' [str [Hinv1 [Hinv2 [Hsnd Hfst]]]]]; subst.
+            apply H3. exists v'. exists (fst x). split_all; auto.
+            simpl_set; triv.
+          -- (*TODO: prev lemma - can we avoid repeating?*)
+            destruct (free_in x (snd (alpha_p_aux sub a0 a1 l))) eqn : Hfree; auto.
+            eapply alpha_p_aux_in_implies in Hfree; [| apply H2 | | |]; auto.
+            ++ exfalso. destruct Hfree.
+              ** destruct H; rewrite Hfreext in H; auto.
+              ** rewrite alpha_p_aux_wf_aux_gen' in H; auto.
+                apply H3. destruct H as [v' [str [Hinv1 [Hinv2 [Hsnd Hfst]]]]]; subst.
+                exists v'. exists (fst x). split_all; auto. 
+                simpl_set; triv.
+                intros; apply Hallin. simpl; simpl_set; triv.
+            ++ intros. apply Hallin. simpl; simpl_set; triv.
+  - destruct H.
+  - inversion Hty; subst.
+    simpl_set.
+    eapply IHp2; [| | | | apply H5]; auto.
+    + intros y Hiny C; apply (Hfree y); auto; simpl; simpl_set; triv.
+    + intros; apply Hallin; simpl; simpl_set; triv.
+    + destruct H; auto. apply H7; auto.
+    + intros [v [str [Hinv1 [Hinv2 [Hsnd Hfst]]]]]; subst.
+      apply H0. exists v. exists (fst x). split_all; auto.
+      simpl. simpl_set; triv.
+  - inversion Hty; subst. 
+    destruct (get_assoc_list vsymbol_eq_dec l v) eqn : Ha.
+    + simpl.
+      simpl_set. destruct H as [Hinx | [Hxv | []]]; subst.
+      * destruct (free_in x (sub v (s, snd v) (snd (alpha_p_aux sub p t l)))) eqn : Hfreex; auto.
+        apply Hsub2 in Hfreex. destruct Hfreex.
+        -- destruct H.
+          eapply alpha_p_aux_in_implies in H; [| apply H6 | | |]; auto.
+          destruct H.
+          ++ destruct H; contradiction.
+          ++ rewrite alpha_p_aux_wf_aux_gen' in H; auto.
+            ** destruct H as [v1 [str [Hinv1 [Hinv2 [Hsnd Hfst]]]]]; subst.
+              exfalso. apply H0. exists v1. exists (fst x).
+              split_all; auto. simpl. simpl_set; triv.
+            ** intros; apply Hallin; simpl; simpl_set; triv.
+          ++ intros; apply Hallin; simpl; simpl_set; triv.
+        -- subst. apply get_assoc_list_some in Ha.
+          exfalso. apply H0. exists v. exists s. split_all; auto.
+          simpl; simpl_set; triv.
+      * rewrite Hsub1; auto. intro; subst.
+        apply H0.
+        apply get_assoc_list_some in Ha.
+        exists x. exists s. split_all; auto. simpl; simpl_set; triv.
+        rewrite H; auto.
+    + simpl. apply get_assoc_list_none in Ha.
+      exfalso. apply Ha. apply Hallin; simpl; simpl_set; triv.
+Qed.
+
+      (*one way: separate induction: prove that if x not in free vars of t
+        AND x not in (map snd l), then x not in free vars of whole thing*)
+      (*this lemma may not hold without assumptions that we cant have repeats*)
+      (*need to think more*)
+  
+  
+  (*assert (In x (big_union vsymbol_eq_dec pat_fv ps) \/ free_in x t = false).
+      left; auto. clear H.
+    generalize dependent t. induction ps; simpl; intros.
+    + destruct H1 as [[] | Hin]; auto.
+    + inversion H0; subst.
+      apply IHps.
+      * intros. intro C. apply (Hfree x0); auto. simpl.
+        simpl in C. rewrite union_elts; right; auto.
+      * intros. apply (Hallin x0). simpl.
+        rewrite union_elts; right; apply H1.
+      * simpl in H.
+        simpl_set. right.
+    
+    
+    simpl in H.
+  
+  revert t.
+  
+  
+  simpl_set.
+
+
+
+      Search alpha_p_aux.
+    simpl.
+      wf_tac.
+
+Check alpha_p_aux.
+
+
+Lemma sub_fv_notin (t: term) (f: formula):
+  (forall (x y: vsymbol),
+    x <> y ->
+    free_in_t x (sub_t x y t) = false)
+
+(*need 2 lemmas: like before
+        1. For any vsymbol in the free vars of p (before),
+          it is NOT free in the result
+        2. For any vsymbol not in the free vars of p before or after,
+          free_in_t is the same as the inderling term*)
+
+(*
+Lemma sub_fv_in (t: term) (f: formula) :
+(forall (x y: vsymbol)
+  (Hbnd: ~ In y (bnd_t t))
+  (Hinx: In x (term_fv t))
+  (Hxy: x <> y),
+  set_eq (term_fv (sub_t x y t))
+  (union vsymbol_eq_dec (remove vsymbol_eq_dec x (term_fv t)) [y])) /\
+  (forall (x y: vsymbol)
+  (Hbnd: ~ In y (bnd_f f))
+  (Hinx: In x (form_fv f))
+  (Hxy: x <> y),
+  set_eq (form_fv (sub_f x y f))
+  (union vsymbol_eq_dec (remove vsymbol_eq_dec x (form_fv f)) [y])).
+Proof.
+Admitted.
+*)
+
+Lemma set_add_remove {A: Type} (eq_dec: forall (x y: A), {x = y} + {x <> y})
+  (l1: list A) (x: A) :
+  In x l1 ->
+  set_eq (union eq_dec (remove eq_dec x l1) [x]) l1.
+Proof.
+  intros; unfold set_eq; intros; simpl_set.
+  split; intros; destruct_all; auto.
+  destruct (eq_dec x x0); subst; triv.
+Qed.
+
+Lemma set_eq_sym {A: Type} (l1 l2: list A):
+  set_eq l1 l2 ->
+  set_eq l2 l1.
+Proof.
+  unfold set_eq; intros. rewrite H; reflexivity.
+Qed.
+
+(*Problem: if we have let t1 := v in t2 and we say sub x with v
+  then v is NOT in the free variables
+  so we need to assume y is not bound*)
+(*
+Lemma sub_t_fv (t: term):
+(forall (x y: vsymbol)
+    (Hbnd: ~ In y (bnd_t t)),
+    set_eq (term_fv (sub_t x y t))
+      (if in_bool vsymbol_eq_dec x (term_fv t) then
+        (union vsymbol_eq_dec (remove vsymbol_eq_dec x (term_fv t)) [y])
+      else term_fv t)).
+Proof.
+  intros. case_in. case (vsymbol_eq_dec x y); intros; subst.
+  - rewrite sub_t_eq. apply set_eq_sym. apply set_add_remove. auto.
+  - apply sub_fv_in; auto. apply Ftrue.
+  - rewrite sub_t_notin; auto. apply set_eq_refl.
+Qed.
+
+Lemma sub_f_fv (f: formula) :
+  (forall (x y: vsymbol)
+    (Hbnd: ~ In y (bnd_f f)),
+    set_eq (form_fv (sub_f x y f))
+      (if in_bool vsymbol_eq_dec x (form_fv f) then
+        (union vsymbol_eq_dec (remove vsymbol_eq_dec x (form_fv f)) [y])
+      else form_fv f)). 
+Proof.
+  intros. case_in. case (vsymbol_eq_dec x y); intros; subst.
+  - rewrite sub_f_eq. apply set_eq_sym. apply set_add_remove. auto.
+  - apply sub_fv_in; auto. apply tm_d.
+  - rewrite sub_f_notin; auto. apply set_eq_refl.
+Qed.*)
+(*
+    
+    
+    rewrite (sub_eq_t). t). subst.
+    apply sub_fv_in; auto.
+  revert t f. apply term_formula_ind; simpl; auto; intros.
+  - apply set_eq_refl.
+  - destruct (vsymbol_eq_dec x v); simpl; apply set_eq_refl.
+  - case_in.
+    + unfold set_eq; intros; simpl_destruct_set.
+      setoid_rewrite in_map_iff.
+      rewrite Forall_forall in H.
+      split; intros; simpl_destruct_set.
+      * apply H in H3; auto. revert H3; case_in; intros.
+        -- simpl_destruct_set; try triv. 
+          left. split; auto. exists x3; auto.
+        -- left. split; [|intro C; subst; contradiction].
+          exists x3; auto.
+        -- intro C. apply Hbnd. rewrite in_concat.
+          exists (bnd_t x3). split; wf_tac.
+      * assert (Hinx1:=H2). apply (H x2) with(x:=x)(y:=y) in H2.
+        revert H2; case_in; intros.
+        -- exists (sub_t x y x2).  split; auto.
+          exists x2; auto.
+          apply H2; simpl_set. triv.
+        -- exists (sub_t x y x2). split; auto. exists x2; auto.
+          apply H2; auto.
+        -- intro C; apply Hbnd; rewrite in_concat; 
+          exists (bnd_t x2); split; wf_tac.
+      * specialize (H _ H0 x x0).
+        exists (sub_t x x0 x1). split; auto.
+        -- exists x1; auto.
+        -- apply H. intro C. apply Hbnd. rewrite in_concat.
+          exists (bnd_t x1); split; wf_tac.
+          destruct (in_bool_spec vsymbol_eq_dec x (term_fv x1)); try contradiction.
+          simpl_set. triv.
+    + unfold set_eq; intros.
+      revert n.
+      (*Could prove this by showing each union identical, see how hard it is to prove otherwise*)
+      simpl_destruct_set; intros.
+      rewrite Forall_forall in H.
+      setoid_rewrite in_map_iff. split; intros; simpl_destruct_set.
+      * apply H in H1; auto.
+        destruct (in_bool_spec vsymbol_eq_dec x (term_fv x2)).
+        -- exfalso. apply n. exists x2; auto.
+        -- exists x2; auto.
+        -- intro C; apply Hbnd; rewrite in_concat; 
+          exists (bnd_t x2); split; wf_tac.
+      * exists (sub_t x y x1). split.
+        -- exists x1; auto.
+        -- apply H; auto.
+          intro C; apply Hbnd; rewrite in_concat; 
+          exists (bnd_t x1); split; wf_tac.
+          destruct (in_bool_spec vsymbol_eq_dec x (term_fv x1)); auto.
+          exfalso. apply n. exists x1; auto.
+  - rewrite in_app_iff in Hbnd. not_or Hbnd.
+    case_in.
+     + unfold set_eq. intros. simpl_destruct_set.
+      * split; intros; simpl_destruct_set.
+        -- apply H in H2; auto. 
+          rewrite (In_in_bool _ _ _ H1) in H2.
+          simpl_destruct_set; triv.
+        -- destruct (vsymbol_eq_dec x v); subst; auto.
+          apply H0 in H2; auto. revert H2; case_in; intros;
+          simpl_destruct_set; triv.
+        -- left. apply H; auto. rewrite (In_in_bool _ _ _ H1).
+            simpl_destruct_set; triv.
+        -- right. destruct (vsymbol_eq_dec x v); auto.
+          split; auto.
+          apply H0; auto. case_in; auto.
+          simpl_destruct_set; triv.
+        -- left.
+          apply H; auto. rewrite (In_in_bool _ _ _ H1).
+          simpl_destruct_set; triv.
+      * destruct (vsymbol_eq_dec x v); subst; try contradiction. clear n.
+        rewrite (H x y Hbnd x0), (H0 x y Hbnd2 x0), (In_in_bool _ _ _ H1).
+        simpl_set.
+        case_in; subst;
+        simpl_set; split; intros; destruct_all; triv.
+    + unfold set_eq; intros. revert n. simpl_set. intros.
+      apply Decidable.not_or in n. destruct n as [Hnotin1 H2].
+      rewrite (H x y Hbnd x0).
+      case_in; try contradiction.
+      clear n.
+      destruct (vsymbol_eq_dec x v); subst; auto; try reflexivity.
+      rewrite (H0 x y Hbnd2 x0).
+      case_in; subst; auto;
+      try reflexivity. exfalso. apply H2; auto.
+  - rewrite !in_app_iff in Hbnd.
+    not_or Hbnd. case_in;
+    unfold set_eq; intros; simpl_destruct_set; 
+    rewrite (H x y Hbnd0 x0), (H0 x y Hbnd x0), (H1 x y Hbnd2 x0);
+    try solve[rewrite (In_in_bool _ _ _ H2); case_in;
+      split; intros; simpl_destruct_set; triv].
+    revert n; simpl_set; intros.
+    not_or Hinfv. case_in; try contradiction; reflexivity.
+  - (*match will be so fun*)
+    rewrite in_app_iff in Hbnd.
+    not_or Hbnd.
+    rewrite in_concat in Hbnd1.
+    setoid_rewrite in_map_iff in Hbnd1.
+    unfold set_eq; intros.
+    case_in.
+    + (*dont do big union for now*) 
+      revert i; rewrite !union_elts, in_remove_iff, !union_elts; intros.
+      rewrite (H x y Hbnd0 x0).
+      destruct i.
+      * case_in; try contradiction. rewrite union_elts, in_remove_iff.
+        split; intros.
+        -- destruct_all. left. split; auto.
+          right. auto.
+          revert H2.
+          rewrite <- !big_union_elts.
+          (*TODO: START HERE*)
+          assert (In x0
+          (big_union vsymbol_eq_dec
+             (fun x1 : pattern * term =>
+              remove_all vsymbol_eq_dec (pat_fv (fst x1)) (term_fv (snd x1)))
+             (map
+                (fun p : pattern * term =>
+                 if in_bool vsymbol_eq_dec x (pat_fv (fst p))
+                 then p
+                 else (fst p, sub_t x y (snd p))) ps)) <->
+        In x0
+          (big_union vsymbol_eq_dec
+             (fun x1 : pattern * term =>
+              remove_all vsymbol_eq_dec (pat_fv (fst x1)) (term_fv (snd x1))) ps)). {
+                rewrite  <- !big_union_elts.
+                split; intros [p1 [Hinp1 Hinx0]].
+                - rewrite in_map_iff in Hinp1. destruct Hinp1 as [p2 [Hp1 Hinx1']]; subst.
+                revert Hinx0. case_in; simpl; intros; exists p2.
+                + split; auto.
+                + (*Here need defn of remove_all*)
+                  split; auto.
+                  simpl_destruct_set. 
+                  rewrite Forall_forall in H0. apply H0 in H2; wf_tac.
+                  revert H2; case_in; intros; simpl_destruct_set; auto.
+                  split; auto. 
+
+
+                  (*HAVE: In x0 (term_fv (sub_t x y (snd p2)))*)
+                  admit.
+                - setoid_rewrite in_map_iff.
+              }
+          (*Can we prove iff for this?*)
+          rewrite <- !big_union_elts.
+
+
+        destruct H2. destruct H2. left.  split; auto. 
+    (*Do *)
+    
+    
+    _iff.
+    case_in; simpl_set.
+    + revert i; simpl_set; intros.
+      rewrite (H x y Hbnd0 x0).
+      split; intros.
+      -- destruct i.
+        ++ revert H1; case_in; try contradiction; intros.
+          destruct H1.
+          ** simpl_destruct_set; triv.
+          ** destruct H1 as [p [Hinp Hinx0]].
+            rewrite in_map_iff in Hinp.
+            destruct Hinp as [p1 [Hp Hinx1']]; subst.
+            revert Hinx0; case_in; intros.
+            {
+              left. split. right. exists p1. auto.
+              intro C; subst.
+              simpl_destruct_set. contradiction.
+            }
+            {
+              simpl_destruct_set; simpl in *.
+              rewrite Forall_forall in H0.
+              apply H0 in H1; wf_tac.
+              2: { intro C; apply Hbnd1. exists (pat_fv (fst p1) ++ bnd_t (snd p1)).
+                split; [exists p1; auto |]. rewrite in_app_iff; auto. }
+              revert H1; case_in; auto; intros. simpl_destruct_set.
+              {
+                left. split; auto. right. exists p1. split; auto.
+                simpl_set. auto.
+              }
+              { right; auto. }
+              { left. split; auto. 2: intro C; subst; contradiction.
+                right. exists p1. split; auto.
+                simpl_set; auto.
+              }
+            }
+        ++ destruct H2 as [p1 [Hinp1 Hinx]].
+          simpl_set. destruct Hinx as [Hinx Hnotinx].
+          simpl_destruct_set.
+          ** revert H1; case_in; intros; simpl_destruct_set; triv.
+          ** rewrite in_map_iff in H1. destruct H1 as [p2 [Hx1 Hinx0]]; subst.
+            revert H3 H2. case_in; simpl_set; simpl; intros.
+            {
+              left. split; [|intro C; subst; contradiction].
+              right. exists p2; simpl. simpl_set. auto.
+            }
+            {
+              rewrite Forall_forall in H0. apply H0 in H2; wf_tac.
+              2: { intro C; apply Hbnd1. exists (pat_fv (fst p2) ++ bnd_t (snd p2)).
+                split; [exists p2; auto|]. rewrite in_app_iff. right; auto. }
+              revert H2; case_in; intros; simpl_destruct_set.
+              {
+                left. split; auto. right. exists p2. simpl_set; auto.
+              }
+              { triv. }
+              {
+                left. split; [|intro C; subst; contradiction].
+                right. exists p2. simpl_set; auto.
+              }
+            }
+      -- rewrite Forall_forall in H0.
+        destruct i.
+        ++ case_in; try contradiction.
+          simpl_set. destruct_all.
+          ** triv.
+          ** right. exists x1. split; auto.
+            rewrite in_map_iff.
+            (*I have no idea wtf is going on*)
+            
+            simpl_destruct_set.
+            right.  
+            right. exists  
+          destruct H1.
+          ** destruct H1. destruct H1.  destruct H1.  
+        
+        
+        simpl_destruct_set; case_in; try contradiction; simpl_set; try triv.
+        ++ right.
+          
+          specialize (H0 H7 x0).
+          unfold set_eq in H0.
+          revert H0.
+          case_in; simpl_set; intros.
+          {
+            specialize (H0 x0).
+
+          }
+
+          exists x1. (*TODO: not this*)
+          rewrite in_map_iff. split. 2: simpl_set; auto.
+          exists x1.
+          revert H0. case_in; unfold set_eq; intros; simpl_set; split; auto.
+
+
+        
+        simpl_set.
+      
+      
+      destruct H1.
+            
+            }
+            triv.
+            simpl_destruct_set.
+            {
+              left. split; auto.
+            }
+        
+        
+        revert H1; case_in; try contradic
+                
+              
+              (*Here, use bound vars assumption*)
+
+              exfalso. apply Hbnd1. exists (pat_fv (fst p1) ++ bnd_t (snd p1)).
+                split; [exists p1; auto|]. 
+                exfalso.
+              }
+              left. split; auto. right; auto. exists p1. split; auto.
+              simpl_set. split; auto.
+              rewrite Forall_forall in H0.
+              apply H0 in H1; auto.
+              { revert H1; case_in; auto; intros.
+                simpl_set. simpl_destruct_set. auto. simpl_destruct_set; auto.
+                exfalso. apply Hbnd1. exists (pat_fv (fst p1) ++ (bnd_t (snd p1))).
+                split. exists p1; auto. apply in_app_iff. left; auto.
+                exists p1. }
+              rewrite <- remove_all_elts in Hinx0. destruct_all; contradiction.
+              simpl in Hinx0.
+              left. split; auto. right. exists p1. split; auto.
+              split.
+              simpl_destruct_set.
+              revert H1 H3. case_in; intros.
+              left. split; [|intro C; subst; contradiction].
+              right. exists p1. split; auto.
+            }
+            
+            }
+            
+            
+            right.
+            split.
+            Search remove_all.
+          
+          revert H1; simpl_destruct_set.
+          left.  split; auto.
+          split; auto.
+      case_in.  left. 2: {  }
+      split; intros.
+      * simpl_destruct_set.
+      * split. left.
+    simpl_set.
+    eapply Classical_Pred_Type.not_ex_all_not in Hbnd1.
+    
+    Print Assumptions Classical_Pred_Type.not_ex_all_not. Search (~ (exists x, ?P x)).
+
+
+
+     (*Now not in anything*)
+      case_in; try [exfalso; apply n; rewrite union_elts]
+      (*TODO: tactic for destructing*)
+
+    
+    simpl_set.
+      
+    
+    simpl_set. 
+
+
+      apply Decidable.not_and in H2. 2: unfold Decidable.decidable.
+      apply Decidable.not_or in H2.
+        split; intros; destruct_all; try triv. left. split. right.  left.
+        right. split; auto. intro; subst.
+        split; auto.
+
+        rewrite H.
+      
+      triv. destruct 9
+      
+      destruct (in_bool_spec vsymbol_eq_dec x (term_fv tm1));
+          apply H0.
+          rewrite (In_in_bool _ _ _ _ H2).
+        
+        
+        left. apply H. rewrite (In_in_bool _ _ _ H2).
+          simpl_destruct_set. triv.
+            
+            destruct (vsymbol_eq_dec x v); subst; auto.
+          ++ 
+          ++ left. apply H. rewrite (In_in_bool _ _ _ H1).
+            simpl_destruct_set; triv. right; split; auto. 
+          left. split_all; auto. intro C; subst.
+          ++ left; split_all; auto.
+          ++ right; auto. left; split_all; auto.   
+  
+  
+  simpl_set.
+      
+      exists x0.  
+        exists 
+
+      
+      
+      Search in_bool In. 
+          apply H; auto.  
+      exists x1. 
+      
+      simpl_destruct_set.
+        
+        rewrite union_elts, in_remove_iff in Hinx0;
+          simpl in Hinx0; rewrite or_false_r.
+          destruct 
+        
+      Search (?P \/ False).
+      split; intros.
+      * destruct H0 as [y' [Hiny' Hinx0]].
+        rewrite in_map_iff in Hiny'. destruct Hiny' as [x1 [Hy' Hinx1]]; subst.
+        rewrite Forall_forall in H.
+        specialize (H _ Hinx1 x y). apply H in Hinx0.
+        destruct (in_bool_spec vsymbol_eq_dec x (term_fv x1)).
+        -- rewrite union_elts in Hinx0. destruct Hinx0; auto.
+          left. rewrite in_remove_iff in H0.
+          rewrite in_remove_iff. destruct H0.
+          split; auto.
+          rewrite <- big_union_elts. exists x1; auto.
+        -- left. rewrite in_remove_iff,<- big_union_elts.
+          split. exists x1; auto.
+          intro C; subst; contradiction.
+      * destruct H0.
+        -- rewrite in_re
+          Search in
+          
+          Search In remove.
+        
+        rewrite union_remove in Hinx0. rewrite remove_union in Hinx0. 
+    
+    
+    unfold union. simpl. simpl. eapply set_eq_trans.
+      * apply set_eq_big_union with(f2:= fun tm => union vsymbol_eq_dec (remove vsymbol_eq_dec x (term_fv tm)) [y])
+        (l2:= l1). wf_tac.
+        rewrite Forall_forall; intros.
+        rewrite in_combine_iff in H0; wf_tac.
+        rewrite Forall_forall in H.
+        destruct H0 as [i [Hi Hx0]].
+        specialize (Hx0 tm_d tm_d); subst; simpl.
+        revert Hi; wf_tac.
+        assert (Hin': In (nth i l1 tm_d) l1) by wf_tac.
+        specialize (H (nth i l1 tm_d) Hin' x y).
+        assert (Hinxi: in_bool vsymbol_eq_dec x (term_fv (nth i l1 tm_d))). {
+
+        } 
+        
+        
+        (map ())))
+        apply H.
+        rewrite map_length; auto.
+      
+      
+      with(l2:=map (union vsymbol_eq_dec (remove vsymbol_eq_dec x (term_fv )))).
+  - 
+    
+    
+    if in_bool vsymbol_eq_dec x (term_fv t) then
+    )
+*)
+*)
+Lemma set_eq_union {A: Type} (eq_dec: forall (x y: A), {x = y} + {x <> y})
+  (l1 l2 l3 l4: list A) :
+  set_eq l1 l2 ->
+  set_eq l3 l4 ->
+  set_eq (union eq_dec l1 l3) (union eq_dec l2 l4).
+Proof.
+  unfold set_eq; intros. simpl_set. rewrite H, H0. reflexivity.
+Qed.
+
+Lemma set_eq_remove {A: Type} (eq_dec: forall (x y: A), {x = y} + {x <> y})
+(l1 l2: list A) x :
+set_eq l1 l2 ->
+set_eq (remove eq_dec x l1) (remove eq_dec x l2).
+Proof.
+  unfold set_eq; intros. simpl_set. rewrite H; reflexivity.
+Qed.
+
+(*If x is not in l already, then remove x (union l [x]) is equal to l*)
+Lemma remove_union_notin  {A: Type} (eq_dec: forall (x y: A), {x = y} + {x <> y})
+(l: list A) x :
+~ In x l ->
+set_eq (remove eq_dec x (union eq_dec l [x])) l.
+Proof.
+  intros. unfold set_eq; intros; simpl_set. split; intros; auto; try triv.
+  destruct_all; auto. contradiction.
+Qed.
+
+Ltac prove_hyp H :=
+  match goal with
+  | H: ?P -> ?Q |- _ => let N := fresh in assert (N: P); [|specialize (H N); clear N]
+  end.
+
+Ltac prove_hyps n H :=
+  match constr:(n) with
+  | O => idtac
+  | (S ?m) => prove_hyp H; [|prove_hyps m H]
+  end.
+  (* 
+  prove_hyp H; [| prove_hyps ]
+  match goal with
+  | H: ?P -> ?Q
+*)
+(*Ugh, of course need assumption that nothing in l appears in fv
+  already*)
+
+Ltac vsym_eq2 x y z :=
+  let H := fresh in
+  assert (H: x = y \/ (x <> y /\ x = z) \/ (x <> y /\ x <> z)) by
+  (vsym_eq x y; right; vsym_eq x z);
+  destruct H as [? | [[? ?]|[? ?]]].
+
+Lemma alpha_aux_fv (t: term) (f: formula) :
+  (forall (ty: vty)
+    (Hty: term_has_type sigma t ty)
+    (l: list string)
+    (Hnodupl: NoDup l)
+    (Hlen: length l = length (bnd_t t))
+    (Hfree: forall x, In (fst x) l -> ~ In x (term_fv t))
+    (Hbnd: forall x, In (fst x) l -> ~ In x (bnd_t t)),
+    forall x,
+    free_in_t x (alpha_t_aux t l) = free_in_t x t) /\
+  (forall 
+    (Hval: valid_formula sigma f)
+    (l: list string)  
+    (Hnodupl: NoDup l)
+    (Hlen: length l = length (bnd_f f))
+    (Hfree: forall x, In (fst x) l -> ~ In x (form_fv f))
+    (Hbnd: forall x, In (fst x) l -> ~ In x (bnd_f f)),
+    forall x,
+    free_in_f x (alpha_f_aux f l) = free_in_f x f).
+Proof.
+  revert t f. apply term_formula_ind; simpl; auto; intros; try reflexivity.
+  - apply existsb_eq; wf_tac.
+    revert H. rewrite !Forall_forall; intros.
+    revert H0. rewrite in_combine_iff; wf_tac.
+    intros [i [Hi Hx]]. specialize (Hx tm_d tm_d).
+    subst; simpl. rewrite map2_nth with(d1:=tm_d)(d2:=nil); wf_tac.
+    assert (term_has_type sigma (nth i l1 tm_d) (nth i (map (ty_subst (s_params f1) l) (s_args f1)) vty_int)).
+    {
+      inversion Hty; subst. rewrite Forall_forall in H10.
+
+      specialize (H10 (nth i l1 tm_d, (nth i (map (ty_subst (s_params f1) l) (s_args f1)) vty_int))).
+      apply H10. rewrite in_combine_iff; wf_tac.
+      exists i. split; auto; intros; f_equal; apply nth_indep; wf_tac. 
+    }
+    eapply H; [| apply H0 | | | |]; wf_tac; intros y Hiny C; apply in_split_lens_ith in Hiny; wf_tac.
+    + apply (Hfree y); simpl_set; auto.
+      exists (nth i l1 tm_d). split; wf_tac.
+    + apply (Hbnd y); auto. rewrite in_concat.
+      exists (bnd_t (nth i l1 tm_d)). split; wf_tac.
+  - (*Let - this case is complicated because we are binding variables*) 
+    destruct l; inversion Hlen.
+    simpl. inversion Hnodupl; subst.
+    inversion Hty; subst.
+    erewrite H; [| apply H9 | | | |]; wf_tac; try(intros y Hiny C); [|apply (Hfree y) | apply (Hbnd y)];
+    try(simpl; right; wf_tac); [|simpl_set; triv|rewrite in_app_iff; triv].
+    f_equal.
+    assert (v <> (s, snd v)). {
+      intro C; subst. apply (Hbnd v); try triv. 
+      left; rewrite C; auto.
+    }
+    specialize (H0 ty H10 (skipn (Datatypes.length (bnd_t tm1)) l)).
+    prove_hyps 4 H0; wf_tac;
+    try(intros y Hiny C); [apply (Hfree y) | apply (Hbnd y)|];
+    try solve[simpl; right; wf_tac];
+    [simpl_set; right; split; auto; intro Heq; subst;
+      apply (Hbnd v); [right; wf_tac | left; auto]
+    | rewrite in_app_iff; triv |].
+    (*Now we proceed by cases depending on whether x = v,
+      x = (s, snd v), or none of the above*)
+    vsym_eq2 x v (s, snd v).
+    + subst. rewrite sub_t_fv_notin; auto. simpl_bool.
+      vsym_eq v v.
+    + (*If x = (s, snd v)*)
+      subst. vsym_eq (s, snd v) (s, snd v).
+      rewrite sub_t_fv_in; auto.
+      * rewrite !H0.
+        vsym_eq (s, snd v) v. simpl.
+        (*TODO: change Hfree to use [free_in_t]?*)
+        symmetry. apply free_in_t_negb. intro Hin.
+        apply (Hfree (s, snd v)). left; auto. 
+        simpl_set. triv.
+      * intro Hin. apply alpha_t_aux_wf in Hin; wf_tac.
+        apply In_skipn in Hin.
+        simpl in Hin. contradiction. (*contradicts NoDup*)
+    + (*The last case is quite easy, nothing changes*) 
+      rewrite sub_t_fv_diff; auto.
+      vsym_eq x (s, snd v); simpl.
+      vsym_eq x v; simpl.
+      apply H0.
+  - (*If case - hypotheses for IH's are annoying *)
+    inversion Hty; subst.
+    rewrite H, (H0 _ H8), (H1 _ H9); wf_tac; intros y Hiny C;
+    [apply (Hfree y) | apply (Hbnd y) | apply (Hfree y) | apply (Hbnd y) |
+    apply (Hfree y) | apply (Hbnd y)];
+    try(apply (Hfree y)); try(apply (Hbnd y));
+    try (apply In_skipn in Hiny); try (apply In_firstn in Hiny);
+    wf_tac; simpl_set; try (rewrite !in_app_iff); triv.
+  - (*Match case - let's see*)
+    inversion Hty; subst.
+    specialize (H _ H4 (firstn (Datatypes.length (bnd_t tm)) l)).
+    prove_hyps 4 H; wf_tac; try(intros y Hiny C);
+    [apply (Hfree y) | apply (Hbnd y) |]; wf_tac;
+    [simpl_set; triv | rewrite in_app_iff; triv |].
+    rewrite H. f_equal.
+    apply existsb_eq; wf_tac.
+    revert H0. rewrite !Forall_forall; intros.
+    revert H1. rewrite in_combine_iff; wf_tac.
+    intros [i [Hi Hx]]. specialize (Hx (Pwild, tm_d) (Pwild, tm_d)).
+    subst; simpl.
+    rewrite map2_nth with(d1:=(Pwild, tm_d))(d2:=nil); wf_tac.
+    assert (Hsum: sum
+    (map
+       (fun x0 : pattern * term =>
+        Datatypes.length (pat_fv (fst x0)) + Datatypes.length (bnd_t (snd x0)))
+       ps) = Datatypes.length l - Datatypes.length (bnd_t tm)). {
+      rewrite Hlen, length_concat, map_map, minus_plus.
+      f_equal. apply map_ext_in_iff; intros.
+        rewrite app_length; auto.
+    }
+    (*Ok, so we are back where we were before*)
+    match goal with
+    | |- context [in_bool ?e ?x ?l] => destruct (in_bool_spec e x l)
+    end; simpl.
+    + (*If x is in the pattern free vars, then it is in l*)
+      destruct (in_bool_spec vsymbol_eq_dec x (pat_fv (fst (nth i ps (Pwild, tm_d))))); simpl; auto.
+      symmetry. apply free_in_t_negb. intro Hinfree.
+      apply alpha_p_aux_wf_aux in i0.
+      * rewrite map_snd_combine in i0; wf_tac.
+        apply In_firstn in i0.
+        apply in_split_lens_ith in i0; wf_tac.
+        apply (Hfree x); wf_tac. simpl_set.
+        right. exists (nth i ps (Pwild, tm_d)).
+        split; wf_tac.
+        simpl_set. split; auto.
+      * rewrite map_fst_combine; wf_tac.
+      * intros. rewrite map_fst_combine; wf_tac.
+    + (*Otherwise, x not in pattern free vars*)
+      (*Need this result in 2 places*)
+      assert (Hnotfree: forall x0 : string * vty,
+      In (fst x0)
+           (nth i
+              (split_lens (skipn (Datatypes.length (bnd_t tm)) l)
+                 (map
+                    (fun x1 : pattern * term =>
+                     Datatypes.length (pat_fv (fst x1)) +
+                     Datatypes.length (bnd_t (snd x1))) ps)) []) ->
+      ~ (In x0 (term_fv (snd (nth i ps (Pwild, tm_d)))) \/
+        In x0 (pat_fv (fst (nth i ps (Pwild, tm_d)))))). {
+        intros y Hy C.
+        apply in_split_lens_ith in Hy; wf_tac.
+        (*Do [pat_fv] first*)
+        assert (~In y (pat_fv (fst (nth i ps (Pwild, tm_d))))). {
+          (*Contradiction: y in l, so not bound in pattern,
+            which is same as pattern free var*)
+          intro Hnot.
+          apply (Hbnd y); wf_tac.
+          rewrite in_app_iff. right.
+          rewrite in_concat. exists (pat_fv (fst (nth i ps (Pwild, tm_d))) ++
+            bnd_t (snd (nth i ps (Pwild, tm_d)))). split; wf_tac.
+          exists (nth i ps (Pwild, tm_d)); split; wf_tac.
+          rewrite in_app_iff; triv.
+        }
+        destruct C; try contradiction.
+        (*Here, contradicts [Hfree], need [pat_fv result]*)
+        apply (Hfree y); simpl_set; wf_tac.
+        right. exists (nth i ps (Pwild, tm_d)). split;
+        auto; simpl_set; wf_tac. 
+      }
+      destruct (in_bool_spec vsymbol_eq_dec x (pat_fv (fst (nth i ps (Pwild, tm_d))))); simpl.
+      * (*If x in orig pattern free vars, need to show false*)
+        assert (Hty': pattern_has_type sigma (fst (nth i ps (Pwild, tm_d))) v). {
+          apply H6. wf_tac.
+        }
+        eapply alpha_p_aux_notin; [apply Hty' | | | | | | |]; wf_tac.
+        -- intros; apply sub_t_fv_notin; auto.
+        -- intros; apply sub_t_in_implies; auto.
+        -- intros. apply In_firstn in H1. apply Hnotfree in H1.
+          intro C; apply H1; triv.
+      * rewrite alpha_p_aux_diff; wf_tac.
+        assert (Hty': term_has_type sigma (snd (nth i ps (Pwild, tm_d))) ty). {
+          apply H8; wf_tac.
+        }
+        -- erewrite H0; [| | apply Hty' | | | |]; wf_tac.
+          ++ intros y Hy C.
+            apply In_skipn in Hy.
+            apply Hnotfree in Hy. apply Hy; triv.
+          ++ intros y Hy C.
+            apply In_skipn in Hy.
+            apply in_split_lens_ith in Hy; wf_tac.
+            apply (Hbnd y); wf_tac.
+            rewrite in_app_iff; right.
+            rewrite in_concat. exists (pat_fv (fst (nth i ps (Pwild, tm_d))) ++
+              bnd_t (snd (nth i ps (Pwild, tm_d)))). split; wf_tac.
+            exists (nth i ps (Pwild, tm_d)); split; wf_tac.
+            rewrite in_app_iff; triv.
+        -- apply sub_t_fv_diff.
+  - (*Teps - basically same as let*) 
+    destruct l; inversion Hlen. inversion Hty; subst. simpl.
+    assert (v <> (s, snd v)). {
+      intro C; subst. apply (Hbnd v); try triv. 
+      left; rewrite C; auto.
+    }
+    inversion Hnodupl; subst.
+    specialize (H H4 l).
+    prove_hyps 4 H; wf_tac;
+    try(intros y Hiny C); [apply (Hfree y) | apply (Hbnd y)|];
+    try solve[simpl; right; wf_tac];
+    simpl_set; auto.
+    split; auto; intro Heq; subst.
+    apply (Hbnd v); [right; wf_tac | left; auto].
+    (*Now we proceed by cases depending on whether x = v,
+      x = (s, snd v), or none of the above*)
+    vsym_eq2 x v (s, snd v).
+    + subst. rewrite sub_f_fv_notin; auto. simpl_bool.
+      vsym_eq v v.
+    + (*If x = (s, snd v)*)
+      subst. vsym_eq (s, snd v) (s, snd v).
+      rewrite sub_f_fv_in; auto.
+      * rewrite !H.
+        vsym_eq (s, snd v) v. simpl.
+        (*TODO: change Hfree to use [free_in_t]?*)
+        symmetry. apply free_in_f_negb. intro Hin.
+        apply (Hfree (s, snd v)). left; auto. 
+        simpl_set. triv.
+      * intro Hin. apply alpha_f_aux_wf in Hin; wf_tac.
+    + (*The last case is quite easy, nothing changes*) 
+      rewrite sub_f_fv_diff; auto.
+      vsym_eq x (s, snd v); simpl.
+      vsym_eq x v; simpl.
+      apply H.
+  - (*All terms done*)
+  
+
+
+    simpl.
+    erewrite H.
+    vsym_eq x (s, snd v).
+    + vsym_eq (s, snd v) v; auto. simpl.
+
+
+
+  forall x0 : string * vty,
+  In (fst x0)
+    (firstn (Datatypes.length (pat_fv (fst (nth i ps (Pwild, tm_d)))))
+       (nth i
+          (split_lens (skipn (Datatypes.length (bnd_t tm)) l)
+             (map
+                (fun x1 : pattern * term =>
+                 Datatypes.length (pat_fv (fst x1)) +
+                 Datatypes.length (bnd_t (snd x1))) ps)) [])) ->
+  ~ In x0 (pat_fv (fst (nth i ps (Pwild, tm_d))))
+
+
+        -- intros. rewrite in_combine_iff in H1; wf_tac.
+          destruct H1 as [j [Hj Hxy]].
+          specialize (Hxy (a, vty_int) a). inversion Hxy.
+          wf_tac.
+        -- rewrite in_map_iff. intro C.
+          destruct C as [y [Hfst Hiny]].
+          apply n.
+          (*Rely on no duplicates*)
+          Search NoDup
+          
+        -- rewrite map_snd_combine; wf_tac.
+          (*TODO: easier to change lemma or prove equivalent?*)
+          intro C.
+          apply n.
+          rewrite alpha_p_aux_wf_aux_gen'; wf_tac.
+          exists (snd x); exists (fst x).
+          Search In pat_fv alpha_p_aux.
+        Check alpha_p_aux_diff.
+          intro 
+          
+          Search free_in_t sub_t.
+
+                simpl_set. right. exists (nth i ps (Pwild, tm_d)).
+                split; wf_tac. simpl_set.
+
+                Search nth split_lens.
+        
+        Search alpha_p_aux pat_fv.
+      (*need 2 lemmas: like before
+        1. For any vsymbol in the free vars of p (before),
+          it is NOT free in the result
+        2. For any vsymbol not in the free vars of p before or after,
+          free_in_t is the same as the inderling term*)
+
+        
+        rewrite in_map_iff in i0.
+        destruct i0 as [y [Hxy Hiny]]; subst.
+        rewrite in_combine_iff in Hiny; wf_tac.
+        -- destruct Hiny as [j [Hj Hy]].
+          specialize (Hy (a, vty_int) a); subst; simpl.
+          rewrite <- Hxy. simpl.
+
+
+
+          destruct x.
+
+      Search pat_fv alpha_p_aux.
+    
+    
+    triv.
+    {
+
+    }
+    
+
+
+    try (apply(Hfree y)); try (apply Hbnd y)
+    + apply (Hfree y); simpl. apply In_skipn in Hiny; wf_tac.
+      simpl_set. triv.
+    + apply (Hbnd y); simpl. apply In_skipn in Hiny; wf_tac.
+      rewrite !in_app_iff; triv.
+    + apply (Hfree y); simpl. apply In_firstn in Hiny; wf_tac.
+      simpl_set. triv.
+    + apply (Hbnd y). apply In_firstn in Hiny; wf_tac.
+      rewrite !in_app_iff; triv.
+    + apply (F)
+      simpl_set. triv. 
+    simpl_set. right. split; auto. intro Heq; subst.
+    apply (Hbnd v). right; wf_tac. left; auto.
+    specialize (H (firstn (Datatypes.length (bnd_f f)) l)
+
+
+        apply (Hbnd (s, snd v)). simpl; triv.
+        rewrite in_app_iff. right. 
+        
+        
+        wf_tac. triv.
+        destruct (free_in_t (s, snd v) tm2) eqn : Hfreet; auto.
+        Search is_true (?x = true).
+        rewrite free_in_t_spec in Hfreet.
+        Search free_in_t.
+    
+    simpl andb.
+    Search free_in_t sub_t.
+
+
+    rewrite H; wf_tac.
+    2: {
+      intros y Hiny C.
+    }
+    
+    wf_tac.
+  
+  
+  apply set_eq_big_union. wf_tac.
+    revert H. rewrite !Forall_forall; intros.
+    revert H0. rewrite in_combine_iff; wf_tac.
+    intros [i [Hi Hx]].
+    specialize (Hx tm_d tm_d).
+    subst. simpl.
+    rewrite map2_nth with(d1:=tm_d)(d2:=nil); wf_tac.
+    apply H; wf_tac; intros x Hinx C; apply in_split_lens_ith in Hinx; wf_tac.
+    + apply (Hfree x); simpl_set; auto.
+      exists (nth i l1 tm_d). split; wf_tac.
+    + apply (Hbnd x); auto. rewrite in_concat.
+      exists (bnd_t (nth i l1 tm_d)). split; wf_tac.
+  - destruct l; inversion Hlen.
+    simpl.
+    apply set_eq_union.
+    + apply H; wf_tac.
+      * inversion Hnodupl; subst; auto. 
+      * intros. intro C. apply (Hfree x); simpl. right; wf_tac.
+        simpl_set. triv.
+      * intros. intro C. apply (Hbnd x). simpl; right; wf_tac.
+        rewrite in_app_iff. triv.
+    + eapply set_eq_trans.
+      apply set_eq_remove.
+      apply sub_t_fv.
+      * intro C. inversion Hnodupl; subst.
+        apply alpha_t_aux_wf in C; wf_tac.
+        apply H4; wf_tac.
+      * (*We use H0 multiple times, so we instantiate the hypotheses*)
+        specialize (H0 ((skipn (Datatypes.length (bnd_t tm1)) l))).
+        inversion Hnodupl; subst.
+        prove_hyps 4 H0; wf_tac.
+        {
+          intros x Hinx C.
+          apply (Hfree x). simpl; right; wf_tac.
+          simpl_set. right. split; auto.
+          intro Heq; subst.
+          apply (Hbnd v). simpl; right; wf_tac. left; auto.
+        }
+        {
+          intros x Hinx C.
+          apply (Hbnd x). simpl; right; wf_tac.
+          rewrite in_app_iff. triv.
+        }
+        case_in.
+        -- eapply set_eq_trans.
+          apply remove_union_notin.
+          simpl_set; intro Hinx.
+          destruct_all.
+          apply H0 in H1.
+          (*contradicts Hfree assumption*) 
+          apply (Hfree (s, snd v)). simpl; auto.
+          simpl_set. triv.
+          apply set_eq_remove. apply H0.
+        -- rewrite !notin_remove; auto.
+          ++ intro C. apply n; apply H0; auto.
+          ++ intro C. apply H0 in C.
+            apply (Hfree (s, snd v)). left; auto.
+            simpl_set. right. split; auto.
+            intro Heq; subst.
+            apply (Hbnd v). left; rewrite <- Heq; auto.
+            left; auto.
+  - (*TODO : if case?*)
+    eapply set_eq_trans.
+    + apply set_eq_union.
+      * apply H; wf_tac.
+        -- intros x Hinx C.
+          apply (Hfree x); wf_tac.
+          simpl_set. triv.
+        -- intros x Hinx C.
+          apply (Hbnd x); wf_tac.
+          rewrite !in_app_iff; triv.
+      * apply set_eq_union.
+        -- apply H0; wf_tac.
+          ++ intros x Hinx C.
+            apply (Hfree x); wf_tac.
+            apply In_firstn in Hinx. wf_tac.
+            simpl_set. triv.
+          ++ intros x Hinx C.
+            apply (Hbnd x); wf_tac.
+            apply In_firstn in Hinx; wf_tac.
+            rewrite !in_app_iff; triv.
+        -- apply H1; wf_tac.
+          ++ intros x Hinx C.
+            apply (Hfree x); wf_tac.
+            apply In_skipn in Hinx; wf_tac.
+            simpl_set. triv.
+          ++ intros x Hinx C.
+            apply (Hbnd x); apply In_skipn in Hinx; wf_tac.
+            rewrite !in_app_iff. triv.
+    + apply set_eq_refl.
+  - (*Pattern case*)
+    apply set_eq_union.
+    { apply H; wf_tac.
+      - intros x Hinx C.
+        apply (Hfree x); wf_tac.
+        simpl_set. triv.
+      - intros x Hinx C.
+        apply (Hbnd x); wf_tac.
+        simpl_set. rewrite in_app_iff. triv.
+    }
+    (*Hmm, can we do it piece by piece? See*)
+    apply set_eq_big_union; wf_tac.
+    revert H0.
+    rewrite !Forall_forall; intros.
+    revert H1. rewrite in_combine_iff; wf_tac.
+    intros [i [Hi Hx]].
+    specialize (Hx (Pwild, tm_d) (Pwild, tm_d)).
+    subst; simpl.
+    rewrite map2_nth with(d1:=(Pwild, tm_d))(d2:=nil); wf_tac.
+    rewrite in_combine_iff in H1.
+    
+    right. exists  triv. }
+            auto. l left; subst; auto. triv.
+        intro C.
+          rewrite <- H0.
+        
+        Search remove In.
+        
+        
+        apply H0; wf_tac.
+            simpl_set. 
+            
+            
+            triv.
+            
+            triv.
+
+
+          assert (Hnodup: NoDup (skipn (Datatypes.length (bnd_t tm1)) l)) by 
+            (inversion Hnodupl; subst; wf_tac).
+          specialize (H0 _ Hnodup).
+          apply H0 in H1; wf_tac.
+          unfold set_eq in Hnodup.
+          apply H0 in Hnodup.
+          rewrite H0 in Hnodup.
+
+          assert (In (s, snd v) (term_fv tm2)). rewrite <- H0.
+
+
+          rewrite (H0 in H1.  
+
+
+
+        apply In_skipn in C 
+      
+      
+      Search bnd_t alpha_t_aux.
+
+
+        wf_tac.
+    (*Need some ext lemmas for union*)
+    
+    rewrite H.
+    + f_equal. (*TODO: not sure about this*) Search term_fv sub_t. rewrite !notin_remove.
+      * f_equal. rewrite H0. Search remove. 
+    
+    
+    H0.
+  
+  unfold big_union.
+  
+  
+  rewrite <- !big_union_elts. split; auto; intros [y [Hiny Hinx]].
+    + rewrite in_map2_iff with(d1:=tm_d)(d2:=nil) in Hiny; wf_tac.
+      destruct Hiny as [i [Hi Hy]]; subst.
+      rewrite Forall_forall in H.
+      apply H in Hinx; wf_tac. exists (nth i l1 tm_d). 
+      split; wf_tac.
+    + eexists.
+      rewrite in_map2_iff with(d1:=tm_d) (d2:=nil); wf_tac. split; auto.
+
+    
+    rewrite Forall_forall in H.
+      apply In_nth with(d:=tm_d) in Hiny.
+      destruct Hiny as [n [Hn Hy]]; subst.
+      exists (nth n l1 tm_d). (*TODO: fix*)
+      rewrite in_map2_iff with(d1:=tm_d) (d2:=nil); wf_tac. split; auto.
+      exists n. split; auto.
+      appl
+      rewrite <- H with(l:=nth n (split_lens l0 (map 
+        (fun tm : term => Datatypes.length (bnd_t tm)) l1)) nil) in Hinx; wf_tac.
+      apply In_nth with(d:=(a, vty_int)) in Hinx.
+      destruct Hinx as [i [Hi Hx]]; subst.
+      exists (nth n )
+      exists (nth)
+      rewrite Hx.
+    
+    
+    exists y. split; auto.
+      rewrite in_map2_iff with(d1:=tm_d)(d2:=nil); wf_tac.
+      rewrite Forall_forall in H.
+      apply In_nth with(d:=tm_d) in Hiny.
+      destruct Hiny as [n [Hn Hnth]]; subst.
+      rewrite <- H with(l:=(nth n
+      (split_lens l0 (map (fun tm : term => Datatypes.length (bnd_t tm)) l1)) nil)) in Hinx; wf_tac.
+      apply In_nth with(d:=(a, vty_int)) in Hinx.
+      destruct Hinx as [i [Hi Hx]]; subst.
+      
+
+      
+      rewrite Forall_forall in H.
+      rewrite <- H with(l:=) in Hinx; wf_tac.
+      exists n. split; auto.
+
+      all: try (apply nth_In; auto).
+      wf 
+
 (*Finally, we need to prove that the [alpha] functions
   do not change the meaning of the term/formula (since we
   only rename bound variables)*)
+
+Context {pd: pi_dom} (all_unif: forall m, mut_in_ctx m gamma -> IndTypes.uniform m)
+  {vt: @val_typevar sigma} {pf: pi_funpred gamma_valid pd}.
+
+Notation term_rep := (term_rep gamma_valid pd all_unif vt pf).
+Notation formula_rep := (formula_rep gamma_valid pd all_unif vt pf).
+
+
+Require Import Coq.Logic.Eqdep_dec.
+
+Lemma alpha_aux_rep (t: term) (f: formula) :
+  (forall (vv: val_vars pd vt) (l: list string) (ty: vty)
+  (Hty: term_has_type sigma t ty)
+  (Hty2: term_has_type sigma (alpha_t_aux t l) ty),
+  NoDup l ->
+  length l = length (bnd_t t) ->
+  term_rep vv t ty Hty =
+  term_rep vv (alpha_t_aux t l) ty Hty2) /\
+  (forall (vv: val_vars pd vt) (l: list string)
+  (Hval: valid_formula sigma f)
+  (Hval2: valid_formula sigma (alpha_f_aux f l)),
+  NoDup l ->
+  length l = length (bnd_f f) ->
+  formula_rep vv f Hval =
+  formula_rep vv (alpha_f_aux f l) Hval2).
+Proof.
+  revert t f; apply term_formula_ind; simpl; intros; auto;
+  try solve[apply term_rep_irrel].
+  - rewrite !tfun_rep.
+    f_equal.
+    apply UIP_dec. apply vty_eq_dec.
+    f_equal. apply UIP_dec. apply sort_eq_dec.
+    (*casting is done*)
+    f_equal.
+    apply get_arg_list_ext; wf_tac.
+    intros i Hi ty' Htya Htyb.
+    revert Htyb.
+    rewrite map2_nth with(d1:=tm_d)(d2:=nil); simpl; intros; wf_tac.
+    rewrite Forall_forall in H; apply H; wf_tac.
+  - destruct l; [apply term_rep_irrel|].
+    inversion H2; subst.
+    inversion H1; subst.
+    assert (Hty3: term_has_type sigma
+    (Tlet (alpha_t_aux tm1 (firstn (Datatypes.length (bnd_t tm1)) l)) v
+       (alpha_t_aux tm2 (skipn (Datatypes.length (bnd_t tm1)) l))) ty). {
+        inversion Hty; subst.
+        constructor; apply alpha_t_aux_type; wf_tac.
+    }
+    rewrite <- alpha_convert_tlet with(Hty1:=Hty3); wf_tac.
+    + rewrite !tlet_rep.
+      rewrite (H vv (firstn (length (bnd_t tm1)) l) (snd v)
+      (proj1 (ty_let_inv (has_type_eq eq_refl Hty)))
+      (proj1 (ty_let_inv (has_type_eq eq_refl Hty2)))); wf_tac.
+      erewrite H0 with(Hty2:=(proj2 (ty_let_inv (has_type_eq eq_refl Hty3)))); wf_tac.
+      erewrite (term_rep_irrel _ _ _ _ _ _ (alpha_t_aux tm1 _)).
+      reflexivity.
+    + intro C. apply alpha_t_aux_wf in C; wf_tac.
+      simpl in C. apply In_skipn in C. contradiction.
+    + intro C.
+      (*TODO: prove that [alpha_t_aux] does not change free variables*)
+    
+    Search term_fv alpha_t_aux. apply alpha_t_aux_wf in C; wf_tac.
+    
+    
+    wf_tac.
+    
+    apply alpha_aux_wf_aux in C; wf_tac.
+    
+    
+    Search alpha_t_aux.
+    
+    reflexivity.
+      erewrite (term_rep_irrel _ _ _ _ _ _ (alpha_t_aux tm2 _)).
+      apply H0.
+    
+
+
+      (term_rep vv (alpha_t_aux tm1 (firstn (Datatypes.length (bnd_t tm1)) l))
+        (snd (s, snd v)) (proj1 (ty_let_inv (has_type_eq eq_refl Hty2)))))
+
+    rewrite H.
+    + wf_tac.
+    rewrite nth_map2.
+    wf_tac.
+    + wf_tac. rewrite map2_length.
+    (*TODO: need another more general [get_arg_list_eq] lemma
+      says: have ts1 and ts2, lengths are the same
+      and forall i, i < length ts1 ->
+      forall ty Hty1 Hty2, reps (nth i ts1 d_tm) ty Hty1 = 
+        reps (nth i ts2 d_tm) ty Hty2 ->
+        get_args_lists eq - so general over ts, reps, Hty*)
+    (*Should work for sub_t/f lemma as well *)
+
+    f_equal.
+
+    Check get_arg_list_eq.
+    apply get_arg_list_eq.
+  
+  
+  apply term_rep_irrel. inversion Hty; subst.
+  
+  /\
+  (Hnodup: NoDup l)
+  (Hlenl: length l = length (bnd_t t)),
+  term_has_type sigma t ty ->
+  term_has_type sigma (alpha_t_aux t l) ty) /\
+  (forall (l: list string)
+  (Hnodup: NoDup l)
+  (Hlenl: length l = length (bnd_f f)),
+  valid_formula sigma f ->
+  valid_formula sigma (alpha_f_aux f l)).
